src/PermArray.v
@@ -1,0 +1,1692 @@
+Require Import Mem.
+Require Import ListUtils.
+Require Import List Omega Ring Word Pred.
+Require Import FunctionalExtensionality.
+Require Import WordAuto.
+Require Export PermPredCrash.
+
+Import ListNotations.
+
+Set Implicit Arguments.
+Set Default Proof Using "Type".
+
+
+(** * A generic array predicate: a sequence of consecutive points-to facts *)
+
+Section GenArray.
+
+  Variable V VP : Type.
+  Variable pts : addr -> V -> @pred addr addr_eq_dec VP.
+
+  Infix "|-?->" := pts (at level 35) : pred_scope.
+
+  Fixpoint arrayN (a : addr) (vs : list V) : @pred _ addr_eq_dec _ :=
+    match vs with
+      | nil => emp
+      | v :: vs' => a |-?-> v * arrayN (S a) vs'
+    end%pred.
+
+  Lemma arrayN_unify : forall (a b : list V) s,
+    a = b -> arrayN s a =p=> arrayN s b.
+  Proof.
+    intros; subst; auto.
+  Qed.
+
+  Lemma arrayN_one: forall v,
+      0 |-?-> v <=p=> arrayN 0 [v].
+  Proof.
+    split; cancel.
+  Qed.
+
+  Lemma isolateN_fwd' : forall vs i a (default : V),
+    i < length vs
+    -> arrayN a vs =p=> arrayN a (firstn i vs)
+       * (a + i) |-?-> selN vs i default
+       * arrayN (a + i + 1) (skipn (S i) vs).
+  Proof.
+    induction vs; simpl; intuition.
+
+    inversion H.
+
+    destruct i; rewrite <- H1 in *; simpl.
+
+    replace (a0 + 0) with (a0) by omega.
+    replace (a0 + 1) with (S a0) by omega.
+    cancel.
+
+    eapply pimpl_trans; [ apply pimpl_sep_star; [ apply pimpl_refl | apply IHvs ] | ]; clear IHvs.
+    eassign i; auto.
+    simpl.
+    replace (S (a0 + i)) with (a0 + S i) by omega.
+    replace (S (a0 + i + 1)) with (a0 + S i + 1) by omega.
+    cancel.
+
+    destruct i; rewrite <- H0 in *; simpl.
+    replace (a0 + 0) with (a0) by omega.
+    replace (a0 + 1) with (S a0) by omega.
+    cancel.
+    
+    eapply pimpl_trans; [ apply pimpl_sep_star; [ apply pimpl_refl | apply IHvs ] | ]; clear IHvs.
+    eassign i; omega.
+    simpl.
+    replace (S (a0 + i)) with (a0 + S i) by omega.
+    replace (S (a0 + i + 1)) with (a0 + S i + 1) by omega.
+    cancel.
+  Qed.
+
+  Theorem isolateN_fwd : forall (default : V) a i vs,
+    i < length vs
+    -> arrayN a vs =p=> arrayN a (firstn i vs)
+       * (a + i) |-?-> selN vs i default
+       * arrayN (a + i + 1) (skipn (S i) vs).
+  Proof.
+    intros.
+    eapply pimpl_trans; [ apply isolateN_fwd' | ].
+    eassumption.
+    apply pimpl_refl.
+  Qed.
+
+  Lemma isolateN_bwd' : forall vs i a (default : V),
+    i < length vs
+    -> arrayN a (firstn i vs)
+       * (a + i) |-?-> selN vs i default
+       * arrayN (a + i + 1) (skipn (S i) vs)
+    =p=> arrayN a vs.
+  Proof.
+    induction vs; simpl; intuition.
+
+    inversion H.
+
+    destruct i; rewrite <- H1 in *; simpl.
+
+    replace (a0 + 0) with (a0) by omega.
+    replace (a0 + 1) with (S a0) by omega.
+    cancel.
+
+    eapply pimpl_trans; [ | apply pimpl_sep_star; [ apply pimpl_refl | apply IHvs ] ]; clear IHvs.
+    2: instantiate (1 := i); omega.
+    simpl.
+    replace (a0 + S i) with (S (a0 + i)) by omega.
+    cancel.
+
+    destruct i; rewrite <- H0 in *; simpl.
+
+    replace (a0 + 0) with (a0) by omega.
+    replace (a0 + 1) with (S a0) by omega.
+    cancel.
+
+    eapply pimpl_trans; [ | apply pimpl_sep_star; [ apply pimpl_refl | apply IHvs ] ]; clear IHvs.
+    2: instantiate (1 := i); omega.
+    simpl.
+    replace (a0 + S i) with (S (a0 + i)) by omega.
+    cancel.
+  Qed.
+
+  Theorem isolateN_bwd : forall (default : V) a i vs,
+    i < length vs
+    -> arrayN a (firstn i vs)
+       * (a + i) |-?-> selN vs i default
+       * arrayN (a + i + 1) (skipn (S i) vs)
+    =p=> arrayN a vs.
+  Proof.
+    intros.
+    eapply pimpl_trans; [ | apply isolateN_bwd' ].
+    2: eassumption.
+    apply pimpl_refl.
+  Qed.
+
+  Theorem arrayN_isolate : forall (default : V) a i vs,
+    i < length vs
+    -> arrayN a vs <=p=>
+       arrayN a (firstn i vs)
+       * (a + i) |-?-> selN vs i default
+       * arrayN (a + i + 1) (skipn (S i) vs).
+  Proof.
+    unfold piff; split.
+    apply isolateN_fwd; auto.
+    apply isolateN_bwd; auto.
+  Qed.
+
+  Theorem isolate_fwd_upd : forall (v : V) a i vs,
+    i < length vs
+    -> arrayN a (updN vs i v) <=p=>
+       arrayN a (firstn i vs)
+       * (a + i) |-?-> v
+       * arrayN (a + i + 1) (skipn (S i) vs).
+  Proof.
+    intros.
+    erewrite arrayN_isolate with (vs:=updN vs i v) (i:=i) (default:=v);
+      autorewrite with lists; auto.
+    unfold piff; split.
+    cancel; autorewrite with lists; cancel.
+    cancel; autorewrite with lists; cancel.
+  Qed.
+
+  Theorem isolateN_bwd_upd : forall (v : V) a i vs,
+    i < length vs
+    -> arrayN a (firstn i vs)
+       * (a + i) |-?-> v
+       * arrayN (a + i + 1) (skipn (S i) vs)
+       =p=> arrayN a (updN vs i v).
+  Proof.
+    intros.
+    erewrite <- isolateN_bwd with (vs:=updN vs i v) (i:=i) (default:=v).
+    rewrite selN_updN_eq by auto.
+    rewrite firstn_updN_oob by auto.
+    rewrite skipN_updN' by auto.
+    cancel.
+    rewrite length_updN.
+    auto.
+  Qed.
+
+  Theorem arrayN_app : forall (a b : list V) st,
+    arrayN st (a ++ b) <=p=>
+    arrayN st a * arrayN (st + length a) b.
+  Proof.
+    induction a; split; simpl; auto.
+    rewrite Nat.add_0_r; cancel.
+    rewrite Nat.add_0_r; cancel.
+    rewrite IHa.
+    replace (S st + length a0) with (st + S (length a0)) by omega.
+    cancel.
+    rewrite IHa.
+    replace (S st + length a0) with (st + S (length a0)) by omega.
+    cancel.
+  Qed.
+
+  Theorem arrayN_split : forall i (a : list V) st,
+    arrayN st a <=p=>
+    arrayN st (firstn i a) * arrayN (st + i) (skipn i a).
+  Proof.
+    intros.
+    destruct (lt_dec i (length a)).
+    erewrite arrayN_isolate; eauto.
+    setoid_rewrite arrayN_isolate with (i := 0) at 4.
+    rewrite skipn_skipn, skipn_selN.
+    replace (st + i + 0) with (st+i) by omega.
+    replace (1 + i) with (S i) by omega.
+    replace (i + 0) with i by omega.
+    split; cancel.
+    rewrite skipn_length.
+    omega.
+    rewrite firstn_oob, skipn_oob by omega.
+    split; cancel.
+    Grab Existential Variables.
+    destruct a.
+    contradict l; simpl; omega.
+    exact v.
+  Qed.
+
+
+  Lemma arrayN_ptsto_selN_0 : forall l (def : V) a,
+    length l = 1 ->
+    arrayN a l <=p=> (a |-?-> selN l 0 def)%pred.
+  Proof.
+    destruct l; simpl; intros; try congruence.
+    assert (length l = 0) by omega.
+    apply length_nil in H0; subst; simpl; split; cancel.
+  Qed.
+
+  Lemma arrayN_isolate_hd : forall l (def : V) a,
+    length l >= 1 ->
+    arrayN a l <=p=> (a |-?-> selN l 0 def * arrayN (a + 1) (skipn 1 l) )%pred.
+  Proof.
+    destruct l; simpl; intros; try omega.
+    replace (a + 1) with (S a) by omega; auto.
+  Qed.
+
+
+End GenArray.
+
+
+
+Section PtstoArray.
+
+  Variable V : Type.
+  Notation pts := (@ptsto addr addr_eq_dec V).
+
+  Lemma arrayN_oob': forall (l : list V) a i m,
+    i >= length l
+    -> arrayN pts a l m
+    -> m (a + i) = None.
+  Proof.
+    induction l; intros; auto; simpl in *.
+    destruct (eq_nat_dec i 0); auto.
+    subst; simpl in *; omega.
+
+    unfold sep_star in H0; rewrite sep_star_is in H0; unfold sep_star_impl in H0.
+    repeat deex.
+    unfold mem_union.
+    unfold ptsto in H2; destruct H2; rewrite H2.
+    pose proof (IHl (S a0) (i - 1)).
+    replace (S a0 + (i - 1)) with (a0 + i) in H3 by omega.
+    apply H3; try omega.
+
+    auto.
+    omega.
+  Qed.
+
+  Lemma arrayN_oob: forall (l : list V) i m,
+    i >= length l
+    -> arrayN pts 0 l m
+    -> m i = None.
+  Proof.
+    intros.
+    replace i with (0 + i) by omega.
+    eapply arrayN_oob'; eauto.
+  Qed.
+
+  Lemma arrayN_oob_lt: forall (l : list V) i a m,
+    arrayN pts a l m ->
+    i < a ->
+    m i = None.
+  Proof.
+    induction l; intros; auto; simpl in *.
+    unfold sep_star in H; rewrite sep_star_is in H; unfold sep_star_impl in H.
+    repeat deex.
+    unfold mem_union.
+    unfold ptsto in H2; destruct H2; rewrite H2.
+    eapply IHl; eauto.
+    omega.
+  Qed.
+
+  Lemma arrayN_updN_memupd : forall F l a i (v : V) m,
+    (F * arrayN pts a l)%pred m ->
+    i < length l ->
+    (F * arrayN pts a (updN l i v))%pred (Mem.upd m (a + i) v).
+  Proof.
+    intros.
+    rewrite arrayN_isolate with (i := i).
+    eapply pimpl_trans; [ apply pimpl_refl | | eapply ptsto_upd ].
+    rewrite selN_updN_eq by auto.
+    cancel.
+    rewrite firstn_updN_oob by auto.
+    rewrite skipn_updN by auto.
+    pred_apply.
+    rewrite arrayN_isolate by eauto.
+    cancel.
+    rewrite length_updN; auto.
+    Grab Existential Variables. all: eauto.
+  Qed.
+
+  Lemma arrayN_app_memupd : forall l (v : V) m,
+    arrayN pts 0 l m
+    -> arrayN pts 0 (l ++ v :: nil) (Mem.upd m (length l) v).
+  Proof.
+    intros.
+
+    eapply isolateN_bwd with (i := (length l)) (default := v).
+    rewrite app_length; simpl; omega.
+
+    rewrite firstn_app2; auto.
+    rewrite selN_last; auto.
+    rewrite skipn_oob; [ | rewrite app_length; simpl; omega ].
+    unfold arrayN at 2; auto; apply emp_star_r.
+    simpl.
+
+    apply ptsto_upd_disjoint; auto.
+    eapply arrayN_oob; eauto.
+  Qed.
+
+
+  Theorem arrayN_list_eq : forall (vs1 vs2 : list V) s m,
+    arrayN pts s vs1 m -> arrayN pts s vs2 m -> vs1 = vs2.
+  Proof.
+    induction vs1; destruct vs2; simpl; intros; auto.
+    apply ptsto_valid in H0; congruence.
+    apply ptsto_valid in H; congruence.
+    apply ptsto_valid in H as Hx.
+    apply ptsto_valid in H0 as Hy.
+    rewrite Hx in Hy; inversion Hy; subst; clear Hx Hy; f_equal.
+    apply ptsto_mem_except in H.
+    apply ptsto_mem_except in H0.
+    eapply IHvs1; eauto.
+  Qed.
+
+  Theorem arrayN_strictly_exact : forall (vs : list V) base,
+    strictly_exact (arrayN pts base vs).
+  Proof.
+    induction vs; simpl; intros.
+    apply emp_strictly_exact.
+    apply sep_star_strictly_exact.
+    apply ptsto_strictly_exact.
+    eauto.
+  Qed.
+
+  Lemma arrayN_selN : forall F a st l m (def : V),
+    (F * arrayN pts st l)%pred m ->
+    a >= st ->
+    a < st + length l ->
+    m a = Some (selN l (a - st) def).
+  Proof.
+    intros.
+    eapply ptsto_valid; pred_apply.
+    rewrite arrayN_isolate with (i := a - st) by omega.
+    replace (st + (a - st)) with a by omega.
+    clear H; cancel.
+  Qed.
+
+  Lemma arrayN_selN_exis : forall F a st (l : list V) m,
+    (F * arrayN pts st l)%pred m ->
+    a >= st ->
+    a < st + length l ->
+    exists v, m a = Some v.
+  Proof.
+    intros; destruct l.
+    simpl in *; try omega.
+    eexists; eapply arrayN_selN with (def := v); eauto; try omega.
+  Qed.
+
+  Lemma arrayN_unify' : forall a b s m (F1 F2 : pred), length a = length b ->
+    (F1 * arrayN pts s a)%pred m -> (F2 * arrayN pts s b)%pred m -> a = b.
+  Proof.
+    induction a as [|x a']; intros.
+    simpl in *.
+    rewrite length_nil; auto.
+    destruct b as [|y b']; simpl in *.
+    inversion H.
+    inversion H.
+    erewrite IHa' with (s := S s); eauto.
+    f_equal.
+    assert (m s = Some x /\ m s = Some y); intuition.
+    all : try match goal with
+      | [ H : (_ * (pts ?s ?x * _))%pred ?m |- ?m ?s = Some ?x] =>
+        eapply ptsto_valid;
+        eapply pimpl_apply; [> | exact H]; cancel
+      | [ H : (_ * (_ * arrayN _ _ ?a))%pred ?m |- (_ * arrayN _ _ ?a)%pred _] =>
+        eapply pimpl_apply; [> | exact H]; cancel
+              end.
+    rewrite H4 in H5; inversion H5; auto.
+  Qed.
+
+End PtstoArray.
+
+Lemma arrayN_piff_replace: forall T V (l : list T) n (p q : _ -> _ -> @pred _ _ V),
+  (forall i d x, i < length l -> selN l i d = x -> p (i + n) x <=p=> q (i + n) x) ->
+  arrayN p n l <=p=> arrayN q n l.
+Proof.
+  induction l; cbn; intros; auto.
+  rewrite H with (i := 0) by (auto; omega).
+  rewrite IHl.
+  split; cancel.
+  intros.
+  rewrite <- plus_Snm_nSm.
+  rewrite H; (eauto; omega).
+Qed.
+
+Lemma arrayN_map: forall V T T' (l : list T) n (p : addr -> T' -> @pred _ _ V) (f : T -> T'),
+  arrayN p n (map f l) <=p=> arrayN (fun i x => p i (f x)) n l.
+Proof.
+  induction l; cbn; intros; auto.
+  rewrite IHl.
+  auto.
+Qed.
+
+Definition vsupd vs i v :=  updN vs i (v, vsmerge (selN vs i valuset0)).
+Definition vssync (vs: list valuset) i :=  updN vs i (fst (selN vs i valuset0), nil).
+
+Definition vsupd_range (vsl : list valuset) vl :=
+  let n := length vl in
+  (List.combine vl (map vsmerge (firstn n vsl))) ++ skipn n vsl.
+
+Definition vs_synced a (vl : list valuset) :=
+  snd (selN vl a valuset0) = nil.
+
+Lemma vsupd_length : forall vsl a v,
+  length (vsupd vsl a v) = length vsl.
+Proof.
+  unfold vsupd; intros.
+  rewrite length_updN; auto.
+Qed.
+
+Lemma vsupd_range_length : forall vsl l,
+  length l <= length vsl ->
+  length (vsupd_range vsl l) = length vsl.
+Proof.
+  unfold vsupd_range; intros.
+  rewrite app_length.
+  rewrite combine_length.
+  rewrite Nat.min_l.
+  rewrite skipn_length.
+  omega.
+  rewrite map_length.
+  rewrite firstn_length_l; auto.
+Qed.
+
+Lemma vsupd_range_nil : forall vsl,
+  vsupd_range vsl nil = vsl.
+Proof.
+  unfold vsupd_range; intros.
+  autorewrite with lists; simpl; auto.
+Qed.
+
+Lemma vsupd_range_progress : forall i vsl l,
+  length l <= length vsl -> i < length l ->
+    (vsupd (vsupd_range vsl (firstn i l)) i (selN l i tagged_block0))
+  = (vsupd_range vsl ((firstn i l) ++ [ selN l i tagged_block0 ])).
+Proof.
+  unfold vsupd, vsmerge; intros.
+  unfold vsupd_range.
+  autorewrite with lists; simpl.
+  repeat replace (length (firstn i l)) with i
+    by (rewrite firstn_length_l by omega; auto).
+  rewrite updN_app2.
+  erewrite firstn_plusone_selN by omega.
+  rewrite map_app.
+  rewrite combine_app
+    by (rewrite map_length; repeat rewrite firstn_length_l; omega).
+  rewrite <- app_assoc; f_equal; simpl.
+  rewrite combine_length; autorewrite with lists.
+  rewrite Nat.min_l; repeat rewrite firstn_length_l; try omega.
+  replace (i - i) with 0 by omega.
+  rewrite updN_0_skip_1 by (rewrite skipn_length; omega).
+  rewrite skipn_skipn'; f_equal; f_equal.
+  rewrite selN_app2.
+  rewrite combine_length; rewrite Nat.min_l;
+     autorewrite with lists; repeat rewrite firstn_length_l; try omega.
+  replace (i + (i - i)) with i by omega.
+  unfold vsmerge; auto.
+  all: rewrite combine_length_eq2; autorewrite with lists;
+    repeat rewrite firstn_length_l; omega.
+Qed.
+
+Lemma forall_incl_refl : forall vs,
+  Forall2 (fun va vb => incl (vsmerge va) (vsmerge vb)) vs vs.
+Proof.
+  induction vs; auto.
+  constructor; auto.
+  apply incl_refl.
+Qed.
+
+
+Lemma vsupd_range_incl : forall l vs,
+  length l <= length vs ->
+  Forall2 (fun va vb => incl (vsmerge va) (vsmerge vb)) vs (vsupd_range vs l).
+Proof.
+  induction l; intros; simpl.
+  rewrite vsupd_range_nil.
+  apply forall_incl_refl.
+
+  destruct vs.
+  inversion H.
+  cbn.
+  constructor.
+  apply incl_tl; apply incl_refl.
+  apply IHl.
+  simpl in *; omega.
+Qed.
+
+
+Lemma vsupd_range_selN_oob : forall vs n l,
+  n >= length l ->
+  length l <= length vs ->
+  selN (vsupd_range vs l) n valuset0 = selN vs n valuset0.
+Proof.
+  unfold vsupd_range; intros.
+  rewrite selN_app2.
+  rewrite combine_length_eq.
+  rewrite skipn_selN.
+  f_equal; omega.
+  rewrite map_length, firstn_length_l; omega.
+  rewrite combine_length_eq; auto.
+  rewrite map_length, firstn_length_l; omega.
+Qed.
+
+Lemma vsupd_range_selN_inb : forall vs n l,
+  n < length l ->
+  length l <= length vs ->
+  selN (vsupd_range vs l) n valuset0 = (selN l n tagged_block0, vsmerge (selN vs n valuset0)).
+Proof.
+  unfold vsupd_range; intros.
+  rewrite selN_app1.
+  unfold valuset0 in *.
+  rewrite selN_combine.
+  erewrite selN_map.
+  rewrite selN_firstn; auto.
+  rewrite firstn_length_l; omega.
+  rewrite map_length, firstn_length_l; auto; omega.
+  rewrite combine_length_eq; auto.
+  rewrite map_length, firstn_length_l; omega.
+Qed.
+
+
+Lemma vsupd_range_firstn_incl : forall n l vs,
+  length l <= length vs ->
+  Forall2 (fun va vb => incl (vsmerge va) (vsmerge vb)) 
+            (vsupd_range vs (firstn n l)) (vsupd_range vs l).
+Proof.
+  induction n; intros.
+  apply vsupd_range_incl; auto.
+  destruct (lt_dec n (length l)).
+
+  erewrite firstn_S_selN by auto.
+  rewrite <- vsupd_range_progress by omega.
+  erewrite <- updN_selN_eq with (l := (vsupd_range vs l)) (ix := n).
+  apply forall2_updN; eauto.
+  rewrite vsupd_range_selN_oob.
+  rewrite vsupd_range_selN_inb; auto; try omega.
+  apply incl_refl.
+  rewrite firstn_length_l; omega.
+  rewrite firstn_length_l; omega.
+
+  rewrite firstn_oob by omega.
+  apply forall_incl_refl.
+Qed.
+
+
+
+Definition vssync_range (vsl : list valuset) n :=
+  (List.combine (map fst (firstn n vsl)) (repeat nil n)) ++ skipn n vsl.
+
+Lemma vssync_range_length : forall vsl n,
+  n <= length vsl ->
+  length (vssync_range vsl n) = length vsl.
+Proof.
+  unfold vssync_range; intros.
+  autorewrite with lists.
+  rewrite combine_length.
+  rewrite Nat.min_l.
+  rewrite skipn_length.
+  autorewrite with lists.
+  rewrite firstn_length_l; omega.
+  autorewrite with lists.
+  rewrite firstn_length_l; omega.
+Qed.
+
+Lemma vssync_range_progress : forall vs m,
+  m < length vs ->
+  vssync (vssync_range vs m) m = vssync_range vs (S m).
+Proof.
+  unfold vssync, vssync_range; intros.
+  rewrite updN_app2.
+  erewrite firstn_S_selN by auto.
+  rewrite map_app.
+  rewrite repeat_app_tail.
+  rewrite combine_app
+    by (autorewrite with lists; rewrite firstn_length_l; omega).
+  rewrite <- app_assoc; f_equal.
+  rewrite combine_length; autorewrite with lists.
+  rewrite Nat.min_l; repeat rewrite firstn_length_l; try omega.
+  replace (m - m) with 0 by omega.
+  rewrite updN_0_skip_1 by (rewrite skipn_length; omega).
+  rewrite skipn_skipn; simpl.
+  f_equal; f_equal.
+  rewrite selN_app2.
+  rewrite combine_length; rewrite Nat.min_l;
+     autorewrite with lists; repeat rewrite firstn_length_l; try omega.
+  replace (m + (m - m)) with m by omega.
+  unfold vsmerge; auto.
+  all: rewrite combine_length_eq2; autorewrite with lists;
+    repeat rewrite firstn_length_l; omega.
+Qed.
+
+
+Lemma vssync_range_incl : forall n vs,
+  n <= length vs ->
+  Forall2 (fun va vb => incl (vsmerge va) (vsmerge vb)) (vssync_range vs n) vs.
+Proof.
+  induction n; simpl; intros.
+  cbn.
+  apply forall_incl_refl.
+  rewrite <- vssync_range_progress by omega.
+  rewrite <- updN_selN_eq with (ix := n) (l := vs) (default := valuset0) at 2.
+  apply forall2_updN.
+  apply IHn; omega.
+
+  unfold vsmerge; simpl.
+  unfold vssync_range.
+  rewrite selN_app2, skipn_selN.
+  rewrite combine_length_eq, map_length, firstn_length_l.
+  rewrite Nat.sub_diag, Nat.add_0_r.
+  apply incl_cons2; apply incl_nil.
+  omega.
+  rewrite map_length, firstn_length_l, repeat_length; omega.
+  rewrite combine_length_eq, map_length, firstn_length_l; try omega.
+  rewrite map_length, firstn_length_l, repeat_length; omega.
+Qed.
+
+
+Definition vsupsyn_range (vsl : list valuset) vl :=
+  let n := length vl in
+  (List.combine vl (repeat nil n)) ++ skipn n vsl.
+
+Lemma vsupsyn_range_length : forall vsl l,
+  length l <= length vsl ->
+  length (vsupsyn_range vsl l) = length vsl.
+Proof.
+  unfold vsupsyn_range; intros.
+  rewrite app_length.
+  rewrite combine_length.
+  rewrite Nat.min_l.
+  rewrite skipn_length.
+  omega.
+  rewrite repeat_length; auto.
+Qed.
+
+Lemma vsupsyn_range_selN : forall vsl vl i def,
+  i < length vl ->
+  selN (vsupsyn_range vsl vl) i (def, nil) = (selN vl i def, nil).
+Proof.
+  unfold vsupsyn_range; intros.
+  rewrite selN_app1.
+  rewrite selN_combine, repeat_selN; auto.
+  rewrite repeat_length; auto.
+  rewrite combine_length_eq; auto.
+  rewrite repeat_length; auto.
+Qed.
+
+Lemma vsupsyn_range_selN_oob : forall vsl vl i def,
+  i >= length vl ->
+  selN (vsupsyn_range vsl vl) i def = selN vsl i def.
+Proof.
+  unfold vsupsyn_range; intros.
+  rewrite selN_app2.
+  rewrite skipn_selN.
+  rewrite combine_length_eq.
+  rewrite le_plus_minus_r; auto.
+  rewrite repeat_length; auto.
+  rewrite combine_length_eq; auto.
+  rewrite repeat_length; auto.
+Qed.
+
+Lemma vsupd_range_app_tl : forall l vs v,
+  length l + 1 <= length vs ->
+  vsupd_range vs (l ++ [v]) = vsupd (vsupd_range vs l) (length l) v.
+Proof.
+  unfold vsupd_range, vsupd; intros.
+  rewrite updN_app2, selN_app2; rewrite combine_length, map_length, firstn_length, Nat.min_l; auto;
+  try apply Nat.min_case_strong; intros; try omega.
+  rewrite Nat.sub_diag, app_length; simpl.
+  erewrite firstn_plusone_selN, map_app by omega.
+  rewrite combine_app by (rewrite map_length, firstn_length_l by omega; auto); simpl.
+  rewrite app_assoc_reverse, updN_0_skip_1, <- cons_app by (rewrite skipn_length; omega).
+  rewrite skipn_skipn', skipn_selN, Nat.add_0_r.
+  reflexivity.
+Qed.
+
+
+(** update vsl according to (addr, valu) pairs in l. *)
+Definition vsupd_vecs (vsl : list valuset) (l : list (addr * tagged_block)) : list valuset :=
+  fold_left (fun vs e => (vsupd vs (fst e) (snd e))) l vsl.
+
+
+Lemma vsupd_vecs_length : forall l vs,
+  length (vsupd_vecs vs l) = length vs.
+Proof.
+  induction l; intros; simpl; auto.
+  rewrite IHl.
+  unfold vsupd.
+  rewrite length_updN; auto.
+Qed.
+
+Lemma vsupd_vecs_length_ok : forall l m def vs,
+  Forall (fun e => fst e < length vs) l ->
+  m < length l ->
+  fst (selN l m def) < length (vsupd_vecs vs (firstn m l)).
+Proof.
+  intros.
+  rewrite vsupd_vecs_length.
+  rewrite Forall_forall in H.
+  apply H.
+  apply in_selN; auto.
+Qed.
+
+Lemma vsupd_vecs_progress : forall l m vs,
+  m < length l ->
+  let e := selN l m (0, tagged_block0) in
+  vsupd (vsupd_vecs vs (firstn m l)) (fst e) (snd e) =
+  vsupd_vecs vs (firstn (S m) l).
+Proof.
+  induction l; intros.
+  inversion H.
+  destruct m; auto.
+  simpl.
+  rewrite IHl; auto.
+  simpl in H.
+  omega.
+Qed.
+
+
+Lemma vsupd_comm : forall l a1 v1 a2 v2,
+  a1 <> a2 ->
+  vsupd (vsupd l a1 v1) a2 v2 = vsupd (vsupd l a2 v2) a1 v1.
+Proof.
+  unfold vsupd; intros.
+  rewrite updN_comm by auto.
+  repeat rewrite selN_updN_ne; auto.
+Qed.
+
+Lemma vsupd_vecs_vsupd_notin : forall av l a v,
+  ~ In a (map fst av) ->
+  vsupd_vecs (vsupd l a v) av = vsupd (vsupd_vecs l av) a v.
+Proof.
+  induction av; simpl; intros; auto.
+  destruct a; simpl in *; intuition.
+  rewrite <- IHav by auto.
+  rewrite vsupd_comm; auto.
+Qed.
+
+Lemma vsupd_vecs_selN_not_in : forall l a d,
+  ~ In a (map fst l) ->
+  selN (vsupd_vecs d l) a valuset0 = selN d a valuset0.
+Proof.
+  induction l; intros; destruct a; simpl in *; auto; intuition.
+  rewrite IHl by auto.
+  unfold vsupd.
+  rewrite selN_updN_ne; auto.
+Qed.
+
+
+Lemma vsupd_vecs_app : forall d a b,
+  vsupd_vecs d (a ++ b) = vsupd_vecs (vsupd_vecs d a) b.
+Proof.
+  unfold vsupd_vecs; intros.
+  rewrite fold_left_app; auto.
+Qed.
+
+Lemma vsupd_vecs_cons : forall l a v avl,
+  vsupd_vecs l ((a, v) :: avl) = vsupd_vecs (vsupd l a v) avl.
+Proof.
+  auto.
+Qed.
+
+
+Lemma vsupd_vecs_selN_vsmerge_in' : forall a v avl l,
+  In v (vsmerge (selN l a valuset0)) ->
+  a < length l ->
+  In v (vsmerge (selN (vsupd_vecs l avl) a valuset0)).
+Proof.
+  intros.
+  destruct (In_dec addr_eq_dec a (map fst avl)).
+  - revert H H0 i; revert avl l a v.
+    induction avl; auto; intros; destruct a.
+    destruct i; simpl in H0; subst.
+
+    destruct (In_dec addr_eq_dec n (map fst avl)).
+    apply IHavl; auto.
+    right; unfold vsupd; simpl.
+    rewrite selN_updN_eq; auto.
+    unfold vsupd; rewrite length_updN; simpl in *; auto.
+
+    rewrite vsupd_vecs_cons, vsupd_vecs_vsupd_notin by auto.
+    unfold vsupd; rewrite selN_updN_eq.
+    rewrite vsupd_vecs_selN_not_in; auto.
+    right; auto.
+    rewrite vsupd_vecs_length; auto.
+
+    rewrite vsupd_vecs_cons.
+    apply IHavl; auto; unfold vsupd.
+    destruct (addr_eq_dec a0 n); subst.
+    rewrite selN_updN_eq; auto.
+    right; auto.
+    rewrite selN_updN_ne; auto.
+    rewrite length_updN; auto.
+  - rewrite vsupd_vecs_selN_not_in; auto.
+Qed.
+
+
+Lemma vsupd_vecs_selN_vsmerge_in : forall a v avl l,
+  In v (vsmerge (selN l a valuset0)) ->
+  In v (vsmerge (selN (vsupd_vecs l avl) a valuset0)).
+Proof.
+  intros.
+  destruct (lt_dec a (length l)).
+  apply vsupd_vecs_selN_vsmerge_in'; auto.
+  rewrite selN_oob in *; auto; try omega.
+  rewrite vsupd_vecs_length; omega.
+Qed.
+
+Lemma vsupd_vecs_incl : forall l vs,
+  Forall (fun e => fst e < length vs) l ->
+  Forall2 (fun va vb => incl (vsmerge va) (vsmerge vb)) vs (vsupd_vecs vs l).
+Proof.
+  intros.
+  eapply selN_Forall2.
+  rewrite vsupd_vecs_length; auto.
+  intros.
+  unfold incl; intros.
+  apply vsupd_vecs_selN_vsmerge_in; eauto.
+Qed.
+
+Lemma vsupd_vecs_firstn_incl : forall n l vs,
+  Forall (fun e => fst e < length vs) l ->
+  Forall2 (fun va vb => incl (vsmerge va) (vsmerge vb)) 
+            (vsupd_vecs vs (firstn n l)) (vsupd_vecs vs l).
+Proof.
+  intros.
+  eapply selN_Forall2 with (da := valuset0) (db := valuset0).
+  repeat rewrite vsupd_vecs_length; auto.
+  repeat rewrite vsupd_vecs_length; auto.
+  intros.
+
+  generalize dependent vs.
+  generalize dependent n.
+  induction l; intros.
+  rewrite firstn_nil; cbn.
+  apply incl_refl.
+  destruct n; simpl.
+  unfold incl; intros.
+  apply vsupd_vecs_selN_vsmerge_in; eauto.
+  cbn.
+  unfold vsupd; destruct a; simpl.
+  destruct (addr_eq_dec n i); subst.
+  rewrite selN_updN_eq; eauto.
+  rewrite selN_updN_ne; eauto.
+
+  apply IHl.
+  rewrite vsupd_length.
+  eapply Forall_cons2; eauto.
+  rewrite vsupd_length; auto.
+Qed.
+
+
+(** sync vsl for all addresses in l. *)
+Definition vssync_vecs (vsl : list valuset) (l : list addr) : list valuset :=
+  fold_left vssync l vsl.
+
+Definition vssync_vecs_rev (vsl : list valuset) (l : list addr) : list valuset :=
+  fold_right (fun a m => vssync m a) vsl (rev l).
+
+Theorem vssync_vecs_rev_eq : forall l vsl,
+  vssync_vecs vsl l = vssync_vecs_rev vsl l.
+Proof.
+  intros; unfold vssync_vecs, vssync_vecs_rev.
+  rewrite fold_left_rev_right; auto.
+Qed.
+
+Lemma vssync_vecs_app : forall m l a,
+  vssync_vecs m (l ++ [a]) = vssync (vssync_vecs m l) a.
+Proof.
+  intros.
+  repeat rewrite vssync_vecs_rev_eq.
+  unfold vssync_vecs_rev.
+  rewrite rev_unit; reflexivity.
+Qed.
+
+Lemma vssync_vecs_length : forall l vs,
+  length (vssync_vecs vs l) = length vs.
+Proof.
+  induction l; intros; simpl; auto.
+  rewrite IHl.
+  unfold vssync.
+  rewrite length_updN; auto.
+Qed.
+
+Lemma vssync_vecs_length_ok : forall l m def vs,
+  Forall (fun e => e < length vs) l ->
+  m < length l ->
+  selN l m def < length (vssync_vecs vs (firstn m l)).
+Proof.
+  intros.
+  rewrite vssync_vecs_length.
+  rewrite Forall_forall in H.
+  apply H.
+  apply in_selN; auto.
+Qed.
+
+Lemma vssync_vecs_progress : forall l m vs,
+  m < length l ->
+  vssync (vssync_vecs vs (firstn m l)) (selN l m 0) =
+  vssync_vecs vs (firstn (S m) l).
+Proof.
+  induction l; intros.
+  inversion H.
+  destruct m; auto.
+  simpl.
+  rewrite IHl; auto.
+  simpl in H.
+  omega.
+Qed.
+
+Lemma vssync_vecs_cons: forall a d x,
+  vssync_vecs d (x :: a) = vssync_vecs (vssync d x) a.
+Proof.
+  auto.
+Qed.
+
+Lemma vssync_vecs_vssync_comm : forall l d a,
+  vssync_vecs (vssync d a) l = vssync (vssync_vecs d l) a.
+Proof.
+  induction l; intros; simpl; auto.
+  destruct (addr_eq_dec a a0); subst; auto.
+  repeat rewrite IHl.
+  unfold vssync.
+  repeat rewrite selN_updN_ne by auto.
+  rewrite updN_comm; auto.
+Qed.
+
+Lemma vssync_vecs_comm: forall l l' vs,
+  vssync_vecs (vssync_vecs vs l) l' = vssync_vecs (vssync_vecs vs l') l.
+Proof.
+  induction l; intros.
+  auto.
+  rewrite vssync_vecs_cons.
+  rewrite IHl.
+  rewrite vssync_vecs_vssync_comm.
+  rewrite vssync_vecs_cons.
+  auto.
+Qed.
+
+Lemma vssync_vecs_app_comm: forall l l' vs,
+  vssync_vecs vs (l ++ l') = vssync_vecs vs (l' ++ l).
+Proof.
+  induction l; intros.
+  rewrite app_nil_r.
+  auto.
+  rewrite <- app_comm_cons.
+  rewrite vssync_vecs_cons.
+  change (a :: l) with ([a] ++ l).
+  rewrite app_assoc.
+  rewrite <- IHl.
+  rewrite app_assoc.
+  rewrite vssync_vecs_app.
+  rewrite vssync_vecs_vssync_comm.
+  auto.
+Qed.
+
+Lemma vssync_vecs_app': forall l l' vs,
+  vssync_vecs (vssync_vecs vs l) l' = vssync_vecs vs (l ++ l').
+Proof.
+  induction l; intros.
+  auto.
+  rewrite <- app_comm_cons.
+  repeat rewrite vssync_vecs_cons.
+  repeat rewrite vssync_vecs_vssync_comm.
+  rewrite IHl; auto.
+Qed.
+
+Lemma vssync_synced : forall l a,
+  vs_synced a l ->
+  vssync l a = l.
+Proof.
+  unfold vs_synced, vssync.
+  intros.
+  rewrite <- H.
+  destruct (lt_dec a (length l)).
+  erewrite selN_inb, <- surjective_pairing by auto.
+  rewrite updN_selN_eq; auto.
+  rewrite updN_oob by omega.
+  auto.
+  Unshelve.
+  apply valuset0.
+Qed.
+
+Lemma vs_synced_vssync_nop: forall vs a,
+  vs_synced a vs -> vssync vs a = vs.
+Proof.
+  unfold vs_synced, vssync.
+  intuition.
+  eapply selN_eq_updN_eq.
+  destruct selN eqn:H'; cbn in *.
+  rewrite H'; congruence.
+Qed.
+
+Lemma vssync_vecs_nop: forall vs l,
+  Forall (fun a => vs_synced a vs) l ->
+  vssync_vecs vs l = vs.
+Proof.
+  induction l; intros.
+  auto.
+  inversion H; subst.
+  rewrite vssync_vecs_cons.
+  rewrite vssync_vecs_vssync_comm.
+  rewrite IHl; auto.
+  eapply vs_synced_vssync_nop; auto.
+Qed.
+
+Lemma vssync_vecs_nil: forall vs,
+  vssync_vecs vs nil = vs.
+Proof.
+  intros.
+  apply vssync_vecs_nop; constructor.
+Qed.
+
+Lemma vssync_comm: forall vs a b,
+  vssync (vssync vs a) b = vssync (vssync vs b) a.
+Proof.
+  intros.
+  unfold vssync.
+  destruct (addr_eq_dec a b); subst; auto.
+  repeat rewrite selN_updN_ne by auto.
+  rewrite updN_comm; auto.
+Qed.
+
+Lemma vssync_vsupd_eq : forall l a v,
+  vssync (vsupd l a v) a = updN l a (v, nil).
+Proof.
+  unfold vsupd, vssync, vsmerge; intros.
+  rewrite updN_twice.
+  destruct (lt_dec a (length l)).
+  rewrite selN_updN_eq; simpl; auto.
+  rewrite selN_oob.
+  repeat rewrite updN_oob by omega; auto.
+  autorewrite with lists; omega.
+Qed.
+
+Lemma updN_vsupd_vecs_notin : forall av l a v,
+  ~ In a (map fst av) ->
+  updN (vsupd_vecs l av) a v = vsupd_vecs (updN l a v) av.
+Proof.
+  induction av; simpl; intros; auto.
+  destruct a; simpl in *; intuition.
+  rewrite IHav by auto.
+  unfold vsupd, vsmerge.
+  rewrite updN_comm by auto.
+  rewrite selN_updN_ne; auto.
+Qed.
+
+
+Lemma vssync_selN_not_in : forall l i d,
+  ~ In i l ->
+  selN (vssync_vecs d l) i valuset0 = selN d i valuset0.
+Proof.
+  induction l; simpl; auto; intuition.
+  rewrite IHl; auto.
+  unfold vssync.
+  rewrite selN_updN_ne; simpl; auto.
+Qed.
+
+
+Lemma vssync_vecs_selN_In : forall l i d,
+  In i l ->
+  i < length d ->
+  selN (vssync_vecs d l) i valuset0 = (fst (selN d i valuset0), nil).
+Proof.
+  induction l; intros; auto.
+  inversion H.
+  destruct (addr_eq_dec a i); subst; simpl.
+  destruct (in_dec addr_eq_dec i l).
+  rewrite IHl; unfold vssync; auto.
+  rewrite selN_updN_eq; simpl; auto.
+  rewrite length_updN; auto.
+
+  rewrite vssync_selN_not_in by auto.
+  unfold vssync; rewrite selN_updN_eq; simpl; auto.
+
+  inversion H; subst; try congruence.
+  rewrite IHl; unfold vssync; auto.
+  rewrite selN_updN_ne; auto.
+  rewrite length_updN; auto.
+Qed.
+
+
+Lemma vssync_vecs_incl : forall l vs,
+  Forall (fun a => a < length vs) l ->
+  Forall2 (fun va vb => incl (vsmerge va) (vsmerge vb)) (vssync_vecs vs l) vs.
+Proof.
+  induction l; simpl; intros.
+  apply forall_incl_refl.
+  rewrite vssync_vecs_vssync_comm.
+  rewrite <- updN_selN_eq with (ix := a) (l := vs) (default := valuset0) at 2.
+  apply forall2_updN.
+  apply IHl; auto.
+  eapply Forall_cons2; eauto.
+
+  destruct (In_dec addr_eq_dec a l).
+  rewrite vssync_vecs_selN_In; auto.
+  unfold vsmerge; simpl.
+  apply incl_cons2; apply incl_nil.
+  inversion H; eauto.
+
+  rewrite vssync_selN_not_in; auto.
+  unfold vsmerge; simpl.
+  apply incl_cons2; apply incl_nil.
+Qed.
+
+
+
+(* crash prediate over arrays *)
+Definition synced_list m: list valuset := List.combine m (repeat nil (length m)).
+
+Definition possible_crash_list l (l': list tagged_block) :=
+  length l = length l' /\
+  forall i, i < length l -> In (selN l' i tagged_block0) (vsmerge (selN l i valuset0)).
+
+Lemma synced_list_selN : forall l i def,
+  selN (synced_list l) i (def, nil) = (selN l i def, nil).
+Proof.
+  unfold synced_list; intros.
+  unfold valuset0, valuset in *.
+  rewrite selN_combine.
+  destruct (lt_dec i (length l)).
+  rewrite repeat_selN; auto.
+  setoid_rewrite selN_oob; auto.
+  omega. rewrite repeat_length; omega. omega.
+  rewrite repeat_length; omega.
+Qed.
+
+Lemma synced_list_map_fst : forall l,
+  map fst (synced_list l) = l.
+Proof.
+  unfold synced_list; intros.
+  rewrite map_fst_combine; auto.
+  rewrite repeat_length; auto.
+Qed.
+
+Lemma vsupsyn_range_synced_list : forall a b,
+  length a = length b ->
+  vsupsyn_range a b = synced_list b.
+Proof.
+  unfold vsupsyn_range, synced_list; intros.
+  rewrite skipn_oob by omega.
+  rewrite app_nil_r; auto.
+Qed.
+
+Lemma possible_crash_list_length : forall l l',
+  possible_crash_list l l' -> length l = length l'.
+Proof.
+  unfold possible_crash_list; firstorder.
+Qed.
+
+Lemma synced_list_length : forall l,
+  length (synced_list l) = length l.
+Proof.
+  unfold synced_list; intros.
+  unfold valuset in *.
+  rewrite combine_length_eq; auto.
+  rewrite repeat_length; auto.
+Qed.
+
+Lemma synced_list_updN : forall l a v,
+  updN (synced_list l) a (v, nil) = synced_list (updN l a v).
+Proof.
+  unfold synced_list; induction l; simpl; intros; auto.
+  destruct a0; simpl; auto.
+  rewrite IHl; auto.
+Qed.
+
+Lemma synced_list_app : forall a b,
+  synced_list (a ++ b) = synced_list a ++ synced_list b.
+Proof.
+  induction a; simpl; auto; intros.
+  unfold synced_list at 1; simpl.
+  f_equal.
+  apply IHa.
+Qed.
+
+Lemma synced_list_inj : forall a b, synced_list a = synced_list b -> a = b.
+Proof.
+  intros.
+  eapply f_equal in H as HH.
+  repeat rewrite synced_list_length in HH.
+  generalize dependent b.
+  induction a; intros; simpl in *.
+  rewrite length_nil; auto.
+  destruct b; simpl in *.
+  inversion HH.
+  unfold synced_list in *.
+  simpl in *.
+  inversion H; f_equal; auto.
+Qed.
+
+Lemma map_snd_synced_list_eq : forall a b,
+  length a = length b ->
+  map snd (synced_list a) = map snd (synced_list b).
+Proof.
+  unfold synced_list; intros.
+  repeat rewrite map_snd_combine; autorewrite with lists; auto.
+Qed.
+
+Lemma map_snd_vsupd_vecs_not_in : forall l d a v,
+  ~ In a (map fst l) ->
+  NoDup (map fst l) ->
+  map snd (vsupd_vecs (synced_list (updN d a v)) l) = map snd (vsupd_vecs (synced_list d) l).
+Proof.
+  induction l; simpl; intros.
+  erewrite map_snd_synced_list_eq; eauto.
+  autorewrite with lists; auto.
+
+  destruct a; intuition; simpl in *.
+  inversion H0; subst.
+  setoid_rewrite vsupd_vecs_vsupd_notin; auto.
+  unfold vsupd.
+  repeat rewrite map_snd_updN.
+  f_equal.
+  apply IHl; auto.
+  f_equal; f_equal; f_equal.
+  rewrite <- synced_list_updN.
+  rewrite <- updN_vsupd_vecs_notin by auto.
+  rewrite selN_updN_ne; auto.
+Qed.
+
+
+Lemma possible_crash_list_updN : forall l l' a v vs,
+  possible_crash_list l l' ->
+  possible_crash_list (updN l a (v, vs)) (updN l' a v).
+Proof.
+  unfold possible_crash_list; simpl; intuition;
+  autorewrite with lists in *; auto.
+  destruct (Nat.eq_dec a i); subst.
+  repeat rewrite selN_updN_eq; auto; omega.
+  repeat rewrite selN_updN_ne; eauto.
+Qed.
+
+
+Lemma possible_crash_list_unique : forall a b,
+  (forall n, snd (selN a n valuset0) = nil) ->
+  possible_crash_list a b ->
+  b = map fst a.
+Proof.
+  unfold possible_crash_list; intuition.
+  eapply list_selN_ext; auto; intros.
+  rewrite map_length; auto.
+  rewrite <- H1 in H0.
+  specialize (H2 _ H0).
+  inversion H2.
+
+  erewrite selN_map; eauto.
+  rewrite H in H3.
+  inversion H3.
+Qed.
+
+Lemma possible_crash_list_synced_list_eq : forall a b,
+  possible_crash_list (synced_list a) b -> a = b.
+Proof.
+  unfold possible_crash_list; intuition.
+  rewrite synced_list_length in *.
+  eapply list_selN_ext; auto; intros.
+  specialize (H1 _ H).
+  inversion H1.
+
+  generalize H2.
+  unfold synced_list, valuset0, valuset in *; rewrite selN_combine; eauto.
+  rewrite repeat_length; auto.
+
+  generalize H2.
+  unfold synced_list, valuset0, valuset in *; rewrite selN_combine; simpl.
+  rewrite repeat_selN by auto.
+  intro Hx; inversion Hx.
+  rewrite repeat_length; auto.
+Qed.
+
+Lemma possible_crash_list_synced_list : forall l,
+  possible_crash_list (synced_list l) l.
+Proof.
+  unfold possible_crash_list; intuition.
+  rewrite synced_list_length; auto.
+  unfold synced_list; constructor.
+  unfold valuset0, valuset in *; rewrite selN_combine; auto.
+  rewrite repeat_length; auto.
+Qed.
+
+Lemma possible_crash_list_cons : forall vsl vl v vs,
+  possible_crash_list vsl vl ->
+  In v (vsmerge vs) ->
+  possible_crash_list (vs :: vsl) (v :: vl).
+Proof.
+  unfold possible_crash_list; intuition.
+  simpl; omega.
+  destruct i, vs, vsl; firstorder.
+Qed.
+
+Theorem possible_crash_list_vssync : forall l l' a,
+  possible_crash_list (vssync l a) l' ->
+  possible_crash_list l l'.
+Proof.
+  unfold possible_crash_list, vssync; intuition; rewrite length_updN in *; auto.
+  specialize (H1 _ H).
+  destruct (addr_eq_dec i a); subst.
+  erewrite selN_updN_eq in H1 by auto; simpl in *. intuition.
+  erewrite selN_updN_ne in H1 by auto; eauto.
+Qed.
+
+
+
+Section ArrayCrashXform.
+
+  Notation pts := (@ptsto addr addr_eq_dec valuset).
+
+  Lemma crash_xform_arrayN: forall l st,
+    crash_xform (arrayN pts st l) =p=>
+      exists l', [[ possible_crash_list l l' ]] *
+      arrayN pts st (synced_list l').
+  Proof.
+    unfold possible_crash_list.
+    induction l; simpl; intros.
+    cancel.
+    instantiate (1 := nil).
+    simpl; auto. auto.
+
+    xform.
+    rewrite IHl.
+    cancel; [ instantiate (1 := v' :: l') | .. ]; simpl; auto; try cancel;
+    destruct i; simpl; auto;
+    destruct (H4 i); try omega; simpl; auto.
+  Qed.
+
+  Lemma crash_xform_arrayN_r: forall l l' st,
+    possible_crash_list l' l ->
+    arrayN pts st (synced_list l) =p=> crash_xform (arrayN pts st l').
+  Proof.
+    unfold possible_crash_list.
+    induction l; simpl; intros; auto.
+    - intuition; destruct l'; simpl in *; try congruence.
+      apply crash_invariant_emp_r.
+    - intuition; destruct l'; simpl in *; try congruence.
+      pose proof (H1 0) as H1'. simpl in H1'.
+      rewrite IHl.
+      rewrite crash_xform_sep_star_dist.
+      rewrite <- crash_xform_ptsto_r with (v := a) by (apply H1'; omega).
+      apply pimpl_refl.
+      intuition.
+      specialize (H1 (S i)). simpl in H1. apply H1. omega.
+  Qed.
+
+  Lemma crash_xform_synced_arrayN: forall l st,
+    Forall (fun x => snd x = nil) l ->
+    crash_xform (arrayN pts st l) =p=> arrayN pts st l.
+  Proof.
+    induction l; simpl; auto; intros.
+    xform.
+    rewrite IHl.
+    cancel; subst.
+    inversion H; simpl in *; subst; auto.
+    inversion H; simpl in *; subst.
+    inversion H1.
+    eapply Forall_cons2; eauto.
+  Qed.
+
+  Lemma crash_xform_arrayN_combine_nils: forall (l : list tagged_block) st,
+    crash_xform (arrayN pts st (List.combine l (repeat nil (length l)))) =p=>
+    arrayN pts st (List.combine l (repeat nil (length l))).
+  Proof.
+    intros.
+    apply crash_xform_synced_arrayN.
+    rewrite Forall_forall; intros.
+    induction l; simpl in *.
+    inversion H.
+    inversion H; subst; simpl; auto.
+  Qed.
+
+  Lemma crash_xform_arrayN_synced: forall (l : list tagged_block) st,
+    crash_xform (arrayN pts st (synced_list l)) =p=>
+    arrayN pts st (List.combine l (repeat nil (length l))).
+  Proof.
+    intros.
+    apply crash_xform_synced_arrayN.
+    rewrite Forall_forall; intros.
+    induction l; simpl in *.
+    inversion H.
+    inversion H; subst; simpl; auto.
+  Qed.
+
+End ArrayCrashXform.
+
+
+
+Section SubsetArray.
+
+  Theorem sync_invariant_arrayN_subset : forall vs a,
+    sync_invariant (arrayN ptsto_subset a vs).
+  Proof.
+    induction vs; simpl; auto.
+  Qed.
+
+  Lemma arrayN_subset_oob': forall l a i m,
+    i >= length l
+    -> arrayN ptsto_subset a l m
+    -> m (a + i) = None.
+  Proof.
+    induction l; intros; auto; simpl in *.
+    destruct (eq_nat_dec i 0); auto.
+    subst; simpl in *; omega.
+
+    unfold sep_star in H0; rewrite sep_star_is in H0; unfold sep_star_impl in H0.
+    repeat deex.
+    unfold mem_union.
+    unfold ptsto_subset in H2.
+    destruct_lift H2.
+    unfold ptsto in H1; destruct H1.
+    pose proof (IHl (S a0) (i - 1)).
+    replace (S a0 + (i - 1)) with (a0 + i) in H3 by omega.
+    destruct (m1 (a0 + i)) eqn:?.
+    contradict Heqo.
+    rewrite H2; try congruence.
+    omega.
+    apply H3.
+    omega.
+    auto.
+  Qed.
+
+
+  Lemma arrayN_subset_oob: forall l i m,
+    i >= length l
+    -> arrayN ptsto_subset 0 l m
+    -> m i = None.
+  Proof.
+    intros.
+    replace i with (0 + i) by omega.
+    eapply arrayN_subset_oob'; eauto.
+  Qed.
+
+   Lemma arrayN_selN_subset : forall F a st l m def,
+    (F * arrayN ptsto_subset st l)%pred m ->
+    a >= st ->
+    a < st + length l ->
+    let vs0 := (selN l (a - st) def) in
+    exists vs, m a = Some vs /\ fst vs = fst vs0 /\ incl (snd vs) (snd vs0).
+  Proof.
+    cbn; intros.
+    rewrite arrayN_isolate with (i := a - st) in H by omega.
+    unfold ptsto_subset at 2 in H; destruct_lift H; simpl in *.
+    eexists; split; try split.
+    eapply ptsto_valid.
+    pred_apply; replace (st + (a - st)) with a by omega.
+    eassign ((fst (selN l (a - st) def), dummy)).
+    cancel.
+    simpl; auto.
+    auto.
+  Qed.
+
+  Lemma arrayN_subset_memupd : forall F l a i v vs vs' m,
+    (F * arrayN ptsto_subset a l)%pred m ->
+    incl vs' vs ->
+    i < length l ->
+    (F * arrayN ptsto_subset a (updN l i (v, vs)))%pred (Mem.upd m (a + i) (v, vs')).
+  Proof.
+    intros.
+    rewrite arrayN_isolate with (i := i) in H by auto.
+    unfold ptsto_subset at 2 in H; destruct_lift H.
+    setoid_rewrite sep_star_comm in H.
+    apply sep_star_assoc in H.
+    apply ptsto_upd with (v := (v, vs')) in H.
+    pred_apply' H.
+    setoid_rewrite arrayN_isolate with (i := i) at 3.
+    unfold ptsto_subset at 4.
+    rewrite selN_updN_eq by auto.
+    cancel.
+    rewrite firstn_updN_oob by auto.
+    rewrite skipn_updN by auto.
+    cancel.
+    rewrite length_updN; auto.
+    Grab Existential Variables. all: apply (v, nil).
+  Qed.
+
+  Lemma crash_xform_arrayN_subset: forall l st,
+    crash_xform (arrayN ptsto_subset st l) =p=>
+      exists l', [[ possible_crash_list l l' ]] *
+      arrayN ptsto_subset st (synced_list l').
+  Proof.
+    unfold possible_crash_list.
+    induction l; simpl; intros.
+    cancel.
+    instantiate (1 := nil).
+    simpl; auto. auto.
+
+    xform.
+    rewrite IHl.
+    rewrite crash_xform_ptsto_subset; unfold ptsto_subset, synced_list.
+    cancel; [ instantiate (1 := v' :: l') | .. ]; simpl; auto; try cancel;
+    destruct i; simpl; auto;
+    destruct (H4 i); try omega; simpl; auto.
+  Qed.
+
+  Lemma crash_xform_arrayN_subset_r: forall l l' st,
+    possible_crash_list l' l ->
+    arrayN ptsto_subset st (synced_list l) =p=>
+     crash_xform (arrayN ptsto_subset st l').
+  Proof.
+    unfold possible_crash_list.
+    induction l; simpl; intros; auto.
+    - intuition; destruct l'; simpl in *; try congruence.
+      apply crash_invariant_emp_r.
+    - intuition; destruct l'; simpl in *; try congruence.
+      pose proof (H1 0) as H1'. simpl in H1'.
+      rewrite IHl.
+      rewrite crash_xform_sep_star_dist.
+      rewrite <- crash_xform_ptsto_subset_r with (v := a) by (apply H1'; omega).
+      rewrite ptsto_subset_pimpl_ptsto.
+      apply pimpl_refl.
+      intuition.
+      specialize (H1 (S i)). simpl in H1. apply H1. omega.
+  Qed.
+
+  Hint Resolve incl_refl.
+
+  Lemma crash_xform_synced_arrayN_subset: forall l st,
+    Forall (fun x => snd x = nil) l ->
+    crash_xform (arrayN ptsto_subset st l) =p=> arrayN ptsto_subset st l.
+  Proof.
+    induction l; simpl; auto; intros.
+    xform.
+    rewrite IHl.
+    cancel; subst.
+    rewrite crash_xform_ptsto_subset; unfold ptsto_subset.
+    cancel.
+    inversion H; simpl in *; subst; auto.
+    inversion H; simpl in *; subst.
+    inversion H0.
+    eapply Forall_cons2; eauto.
+  Qed.
+
+  Lemma crash_xform_arrayN_subset_combine_nils: forall (l : list tagged_block) st,
+    crash_xform (arrayN ptsto_subset st (List.combine l (repeat nil (length l)))) =p=>
+    arrayN ptsto_subset st (List.combine l (repeat nil (length l))).
+  Proof.
+    intros.
+    apply crash_xform_synced_arrayN_subset.
+    rewrite Forall_forall; intros.
+    induction l; simpl in *.
+    inversion H.
+    inversion H; subst; simpl; auto.
+  Qed.
+
+  Lemma crash_xform_arrayN_subset_synced: forall (l : list tagged_block) st,
+    crash_xform (arrayN ptsto_subset st (synced_list l)) =p=>
+    arrayN ptsto_subset st (List.combine l (repeat nil (length l))).
+  Proof.
+    intros.
+    apply crash_xform_synced_arrayN_subset.
+    rewrite Forall_forall; intros.
+    induction l; simpl in *.
+    inversion H.
+    inversion H; subst; simpl; auto.
+  Qed.
+
+End SubsetArray.
+
+
+Hint Resolve sync_invariant_arrayN_subset.
+Notation arrayS := (arrayN ptsto_subset).
+
+
+Section ListUpd.
+
+  Variable V : Type.
+  Notation pts := (@ptsto addr addr_eq_dec V).
+
+  Fixpoint listupd (m : @mem _ addr_eq_dec V) base (vs : list V) :=
+    match vs with
+    | nil => m
+    | v :: tl => listupd (upd m base v) (S base) tl
+    end.
+
+  Lemma arrayN_listupd: forall l (m : @mem _ _ V) l0 base F,
+    (F * arrayN pts base l0 )%pred m ->
+    length l0 = length l ->
+    (F * arrayN pts base l)%pred (listupd m base l).
+  Proof.
+    induction l; intros; destruct l0; simpl in *; auto; try omega.
+    apply sep_star_assoc.
+    eapply IHl with (l0 := l0); eauto.
+    setoid_rewrite sep_star_comm at 1.
+    apply sep_star_assoc.
+    eapply ptsto_upd.
+    pred_apply; cancel.
+  Qed.
+
+  Lemma arrayN_listupd_eq : forall (l : list V) F st d,
+    (F * arrayN pts st l)%pred d ->
+    d = listupd d st l.
+  Proof.
+    induction l; simpl; intros; auto.
+    erewrite <- IHl.
+    rewrite upd_nop; auto.
+    eapply ptsto_valid.
+    pred_apply; cancel.
+    rewrite upd_nop; auto.
+    pred_apply; cancel.
+    eapply ptsto_valid.
+    pred_apply; cancel.
+  Qed.
+
+  Lemma listupd_sel_oob : forall (l : list V) a off m,
+    a < off \/ a >= off + (length l) ->
+    listupd m off l a = m a.
+  Proof.
+    induction l; simpl; intros; auto.
+    rewrite IHl by (intuition omega).
+    destruct (addr_eq_dec off a0); subst.
+    exfalso; intuition.
+    rewrite Mem.upd_ne; auto.
+  Qed.
+
+  Lemma listupd_sel_inb : forall (l : list V) a off m def,
+    a >= off ->
+    a < off + (length l) ->
+    listupd m off l a = Some (selN l (a - off) def).
+  Proof.
+    induction l; simpl; intros; try omega.
+    case_eq (a0 - off); intros.
+    replace off with a0 in * by omega.
+    rewrite listupd_sel_oob; intuition.
+    apply Mem.upd_eq; auto.
+
+    erewrite IHl; try omega.
+    replace (a0 - S off) with n by omega; auto.
+  Qed.
+
+  Lemma listupd_sel_cases : forall (l : list V) a off m def,
+    ((a < off \/ a >= off + (length l)) /\ listupd m off l a = m a ) \/
+    (a >= off /\ a < off + (length l) /\ listupd m off l a = Some (selN l (a - off) def) ).
+  Proof.
+    intros.
+    destruct (lt_dec a off);
+    destruct (ge_dec a (off + (length l)));
+    try ( left; intuition; apply listupd_sel_oob; auto ).
+    right; intuition.
+    apply listupd_sel_inb; omega.
+  Qed.
+
+End ListUpd.
+
+
+Section ListUpdSubset.
+
+  Lemma arrayN_listupd_subset : forall l m l0 base F,
+    (F * arrayN ptsto_subset base l0 )%pred m ->
+    length l0 = length l ->
+    (F * arrayN ptsto_subset base l)%pred (listupd m base l).
+  Proof.
+    induction l; intros; destruct l0; simpl in *; auto; try omega.
+    apply sep_star_assoc.
+    eapply IHl with (l0 := l0); eauto.
+    setoid_rewrite sep_star_comm at 1.
+    apply sep_star_assoc.
+    apply sep_star_comm; destruct a, v.
+    eapply ptsto_subset_upd.
+    pred_apply; cancel.
+    apply incl_refl.
+  Qed.
+
+End ListUpdSubset.
