src/PermAsyncRecArray.v
@@ -1,0 +1,662 @@
+Require Import Arith.
+Require Import Bool.
+Require Import Pred.
+(*
+Require Import PermProg.
+Require Import PermHoare.
+Require Import PermSepAuto.
+Require Import PermInstr.
+*)
+Require Import Omega.
+Require Import Word.
+Require Import Rec.
+Require Import WordAuto.
+Require Import Rounding.
+Require Import List ListUtils.
+Require Import Psatz. 
+Require Import Classes.SetoidTactics.
+Require Export PermCacheSec PermRecArrayUtils.
+
+Import ListNotations.
+
+Set Implicit Arguments.
+
+
+(* RecArray on raw, async disk *)
+
+Module AsyncRecArray (RA : RASig).
+
+  Module Defs := RADefs RA.
+  Import RA Defs.
+
+  Definition items_valid xp start (items : itemlist) :=
+    xparams_ok xp /\  start <= (RALen xp) /\
+    Forall Rec.well_formed items /\
+    length items <= (RALen xp - start) * items_per_val.
+
+  (** rep invariant *)
+  Inductive state : Type :=
+  | Synced : list tag -> itemlist -> state
+  | Unsync : list tag -> itemlist -> state
+  .
+  
+  Definition rep_common xp start items tl (vl: list tagged_block) (vsl : list (list tagged_block)) :=
+    items_valid xp start items /\
+    eqlen tl (ipack items) /\
+    vl = combine tl (ipack items) /\ eqlen vl vsl.
+
+  Definition synced_array xp start items tl :=
+    (exists (vl: list tagged_block) vsl, [[ rep_common xp start items tl vl vsl /\
+        vsl = nils (length vl) ]] *
+    arrayS ((RAStart xp ) + start) (combine vl vsl))%pred.
+
+  Definition unsync_array xp start items tl :=
+    (exists vl vsl, [[ rep_common xp start items tl vl vsl ]] *
+    arrayS ((RAStart xp ) + start) (combine vl vsl))%pred.
+
+  Definition array_rep xp start (st : state) :=
+   (match st with
+    | Synced tags items => synced_array xp start items tags
+    | Unsync tags items => unsync_array xp start items tags
+    end)%pred.
+
+  Definition avail_rep xp start nr : rawpred :=
+    (exists vsl, [[ length vsl = nr ]] *
+     arrayS ((RAStart xp) + start) vsl)%pred.
+
+  Definition nr_blocks st :=
+    match st with
+    | Synced _ l => (divup (length l) items_per_val)
+    | Unsync _ l => (divup (length l) items_per_val)
+    end.
+
+  Lemma items_valid_app : forall xp st a b,
+    items_valid xp st (a ++ b) ->
+    items_valid xp st a /\ items_valid xp st b.
+  Proof.
+    unfold items_valid; intros; split; intros;
+    pose proof (well_formed_app_iff itemtype a b);
+    rewrite app_length in *; intuition.
+  Qed.
+
+  Lemma le_add_helper: forall a b c d,
+    b <= d -> a + d <= c -> a + b <= c.
+  Proof.
+    intros; omega.
+  Qed.
+
+  Lemma le_add_le_sub : forall a b c,
+    a <= c -> b <= c - a -> a + b <= c.
+  Proof.
+    intros. omega.
+  Qed.
+
+  Lemma items_valid_app2 : forall xp st a b,
+    length b <= (roundup (length a) items_per_val - length a)
+    -> items_valid xp st a
+    -> Forall Rec.well_formed b
+    -> items_valid xp st (a ++ b).
+  Proof.
+    unfold items_valid, roundup; intuition.
+    pose proof (well_formed_app_iff itemtype a b); intuition.
+    rewrite app_length.
+    eapply le_add_helper. apply H.
+    rewrite le_plus_minus_r.
+    apply mult_le_compat_r.
+    apply divup_le; lia.
+    apply roundup_ge.
+    apply items_per_val_gt_0.
+  Qed.
+
+  Lemma items_valid_app3 : forall xp st a b na,
+    length a = na * items_per_val ->
+    items_valid xp st (a ++ b) -> items_valid xp (st + na) b.
+  Proof.
+    unfold items_valid; intros; split; intros;
+    pose proof (well_formed_app_iff itemtype a b);
+    rewrite app_length in *; intuition.
+
+    apply le_add_le_sub; auto.
+    eapply Nat.mul_le_mono_pos_r.
+    apply items_per_val_gt_0.
+    rewrite <- H; omega.
+
+    rewrite Nat.sub_add_distr.
+    rewrite Nat.mul_sub_distr_r.
+    apply Nat.le_add_le_sub_l.
+    setoid_rewrite <- H; auto.
+  Qed.
+
+  Lemma items_valid_app4 : forall xp st a b na,
+    length a = na * items_per_val ->
+    items_valid xp st a ->
+    items_valid xp (st + na) b ->
+    items_valid xp st (a ++ b).
+  Proof.
+    unfold items_valid, roundup; intuition.
+    apply well_formed_app_iff; intuition.
+    rewrite app_length.
+    rewrite Nat.sub_add_distr in H8.
+    rewrite Nat.mul_sub_distr_r in H8.
+    rewrite <- H in H8.
+    omega.
+  Qed.
+
+  Lemma synced_array_is : forall xp start items tags,
+    synced_array xp start items tags =p=>
+    arrayS ((RAStart xp) + start) (combine (combine tags (ipack items)) (nils (length (ipack items)))).
+  Proof.
+    unfold synced_array, rep_common; cancel; subst; auto.
+    setoid_rewrite combine_length.
+    rewrite min_r; auto.
+    rewrite H; auto.
+  Qed.
+
+  Lemma array_rep_sync_nil : forall xp a,
+    xparams_ok xp -> a <= (RALen xp) ->
+    array_rep xp a (Synced nil nil) <=p=> emp.
+  Proof.
+    unfold array_rep, synced_array, rep_common; intros.
+    split; cancel; subst; simpl; unfold items_valid, eqlen;
+      try setoid_rewrite ipack_nil; simpl; intuition; auto.
+  Qed.
+
+  Lemma array_rep_sync_nil_emp : forall xp a,
+    array_rep xp a (Synced nil nil) =p=> emp.
+  Proof.
+    unfold array_rep, synced_array, rep_common; intros.
+    cancel; subst; simpl; unfold items_valid, eqlen;
+      try setoid_rewrite ipack_nil; simpl; intuition; auto.
+  Qed.
+
+  Lemma array_rep_sync_nil_sep_star : forall xp a tl l,
+    array_rep xp a (Synced tl l) =p=> array_rep xp a (Synced nil nil) * array_rep xp a (Synced tl l).
+  Proof.
+    intros.
+    unfold array_rep, synced_array, rep_common, eqlen; intros.
+    norm.
+    eassign (@nil tagged_block).
+    cancel.
+    subst; repeat setoid_rewrite ipack_nil; simpl; auto;
+    unfold items_valid in *; intuition.
+    rewrite nils_length; auto.
+  Qed.
+
+  Theorem sync_invariant_array_rep : forall xp a st,
+    sync_invariant (array_rep xp a st).
+  Proof.
+    unfold array_rep, synced_array, unsync_array; destruct st; eauto.
+  Qed.
+
+  Theorem sync_invariant_avail_rep : forall xp a n,
+    sync_invariant (avail_rep xp a n).
+  Proof.
+    unfold avail_rep; eauto.
+  Qed.
+
+  Hint Resolve sync_invariant_array_rep sync_invariant_avail_rep.
+
+  Hint Rewrite list_chunk_nil ipack_nil.
+  Hint Rewrite Nat.add_0_r Nat.add_0_l.
+  Hint Rewrite synced_array_is.
+  Hint Rewrite combine_length nils_length : lists.
+  Hint Rewrite ipack_length divup_mul.
+
+  Ltac rewrite_ignore H :=
+    match type of H with
+    | forall _, corr2 _ _ => idtac
+    | sep_star _ _ _ => idtac
+    end.
+
+  Ltac simplen_rewrite H := try progress (
+    set_evars_in H; (rewrite_strat (topdown (hints core)) in H); subst_evars;
+      [ try simplen_rewrite H | try autorewrite with core .. ];
+    match type of H with
+    | context [ length (list_chunk _ _ _) ] => rewrite block_chunk_length in H
+    end).
+
+  Ltac simplen' := repeat match goal with
+    | [H : @eqlen _ ?T ?a ?b |- context [length ?a] ] => setoid_replace (length a) with (length b) by auto
+    | [H : context[length ?x] |- _] => progress ( first [ is_var x | rewrite_ignore H | simplen_rewrite H ] )
+    | [H : length ?l = _  |- context [ length ?l ] ] => setoid_rewrite H
+    | [H : ?l = _  |- context [ ?l ] ] => setoid_rewrite H
+    | [H : ?l = _ , H2 : context [ ?l ] |- _ ] => rewrite H in H2
+    | [H : @length ?T ?l = 0 |- context [?l] ] => replace l with (@nil T) by eauto
+    | [H : @eqlen _ ?T ?l nil |- context [?l] ] => replace l with (@nil T) by eauto
+    | [ |- _ < _ ] => try solve [eapply lt_le_trans; eauto; try omega ]
+    end.
+
+  Ltac simplen := unfold eqlen; eauto; repeat (try subst; simpl;
+    auto; simplen'; autorewrite with core lists); simpl; eauto; try omega.
+
+  Lemma xform_synced_array : forall xp st l tl,
+    crash_xform (synced_array xp st l tl) =p=> synced_array xp st l tl.
+  Proof.
+    unfold synced_array; intros.
+    xform; cancel; subst.
+    rewrite crash_xform_arrayN_subset_combine_nils.
+    cancel.
+    auto.
+  Qed.
+
+  Lemma xform_synced_rep : forall xp st tl l,
+    crash_xform (array_rep xp st (Synced tl l)) =p=> array_rep xp st (Synced tl l).
+  Proof.
+    intros; simpl.
+    apply xform_synced_array.
+  Qed.
+
+  Lemma xform_avail_rep : forall xp st nr,
+    crash_xform (avail_rep xp st nr) =p=> avail_rep xp st nr.
+  Proof.
+    unfold avail_rep; intros; intros.
+    xform.
+    rewrite crash_xform_arrayN_subset; cancel.
+    unfold possible_crash_list in *; subst; intuition.
+    setoid_rewrite H0.
+    replace (combine l' (repeat [] (length l'))) with (synced_list l') by auto.
+    rewrite synced_list_length; auto.
+  Qed.
+
+
+  Lemma xform_avail_rep_array_rep : forall xp st nr,
+    (forall l', Forall (@Rec.well_formed itemtype) l') ->
+    nr * items_per_val <= (RALen xp - st) * items_per_val ->
+    xparams_ok xp ->
+    st <= RALen xp ->
+    crash_xform (avail_rep xp st nr) =p=>
+      exists l tl, array_rep xp st (Synced tl l) *
+      [[ length l = (nr * items_per_val)%nat ]].
+  Proof.
+    unfold avail_rep; intros.
+    xform.
+    rewrite crash_xform_arrayN_subset; cancel;
+    apply possible_crash_list_length in H3 as Hlength; subst.
+    unfold possible_crash_list in *; subst; intuition.
+    eassign (map fst l').
+    unfold synced_array.
+    cancel.
+    unfold rep_common; intuition.
+    eassign (fold_left iunpack (map snd l') []).
+    unfold items_valid; intuition.
+    rewrite fold_left_iunpack_length.
+    rewrite map_length; setoid_rewrite <- Hlength; auto.
+    
+    rewrite <- ipack_iunpack; auto.
+
+    unfold eqlen.
+    repeat rewrite map_length; eauto.
+
+    rewrite <- ipack_iunpack; auto.
+
+    symmetry; apply combine_map_fst_snd.
+
+    unfold eqlen; rewrite nils_length; auto.
+    rewrite fold_left_iunpack_length.
+    rewrite map_length. setoid_rewrite Hlength; auto.
+  Qed.
+
+  Lemma xform_unsync_array_avail : forall xp st l tl,
+    crash_xform (unsync_array xp st l tl) =p=>
+      avail_rep xp st (divup (length l) items_per_val).
+  Proof.
+    unfold unsync_array, avail_rep, rep_common; intros.
+    xform.
+    rewrite crash_xform_arrayN_subset.
+    unfold possible_crash_list.
+    cancel.
+    rewrite combine_length_eq in *; simplen.
+    rewrite <- ipack_length; auto.
+    setoid_rewrite combine_length in H1; auto.
+    unfold eqlen in *; rewrite min_r in H1; auto.
+    rewrite synced_list_length; auto.
+    rewrite H0; auto.
+  Qed.
+
+  Lemma array_rep_size_ok : forall m xp start st,
+    array_rep xp start st m ->
+    nr_blocks st <= RALen xp - start.
+  Proof.
+    unfold array_rep, synced_array, unsync_array, rep_common, items_valid.
+    destruct st; intros; destruct_lift H; subst;
+    apply divup_le; rewrite Nat.mul_comm; eauto.
+  Qed.
+
+  Lemma array_rep_size_ok_pimpl : forall xp st,
+    array_rep xp 0 st =p=>
+    array_rep xp 0 st * [[ nr_blocks st <= RALen xp ]].
+  Proof.
+    intros; unfold pimpl; intros.
+    apply array_rep_size_ok in H as H1.
+    pred_apply; cancel.
+  Qed.
+
+  Lemma array_rep_avail : forall xp start st,
+    array_rep xp start st =p=>
+    avail_rep xp start (nr_blocks st).
+  Proof.
+    unfold array_rep, avail_rep, synced_array, unsync_array, rep_common, eqlen, nr_blocks.
+    intros; destruct st; cancel; subst; autorewrite with lists.
+    setoid_rewrite combine_length; auto.
+    subst; rewrite min_l; auto.
+    setoid_rewrite combine_length; auto.
+    subst; rewrite min_r; auto.
+    rewrite ipack_length; auto.
+    rewrite H; auto.
+    rewrite H5; auto.
+    rewrite nils_length at 2; auto.
+    rewrite <- ipack_length.
+    setoid_rewrite combine_length.
+    rewrite Nat.min_l; simplen.
+    rewrite <- H4.
+    setoid_rewrite combine_length.
+    rewrite min_r; simplen; auto.
+  Qed.
+
+  Lemma array_rep_avail_synced : forall xp start tags items,
+    array_rep xp start (Synced tags items) =p=>
+    avail_rep xp start (divup (length items) items_per_val).
+  Proof.
+    intros; apply array_rep_avail.
+  Qed.
+
+  Lemma avail_rep_split : forall xp start nr n1 n2,
+    n1 + n2 = nr ->
+    avail_rep xp start nr =p=> avail_rep xp start n1 * avail_rep xp (start + n1) n2.
+  Proof.
+    unfold avail_rep; intros; norm.
+    instantiate (2 := (firstn n1 vsl)).
+    instantiate (1 := (skipn n1 vsl)).
+    cancel.
+    rewrite Nat.add_assoc.
+    rewrite arrayN_split by auto.
+    eassign n1.
+    cancel.
+    intuition.
+    rewrite firstn_length.
+    rewrite Nat.min_l; omega.
+    rewrite skipn_length.
+    omega.
+  Qed.
+
+  Lemma avail_rep_merge : forall xp start nr n1 n2,
+    n1 + n2 = nr ->
+    avail_rep xp start n1 * avail_rep xp (start + n1) n2 =p=> avail_rep xp start nr.
+  Proof.
+    unfold avail_rep; intros; norm.
+    instantiate (1 := vsl ++ vsl0).
+    setoid_rewrite arrayN_app.
+    rewrite Nat.add_assoc.
+    cancel.
+    intuition.
+    rewrite app_length; omega.
+  Qed.
+
+  Lemma helper_add_sub : forall a b c,
+    b <= c -> c <= a -> a >= b + (a - c).
+  Proof.
+    intros; omega.
+  Qed.
+
+  Lemma helper_add_le : forall a b nb n,
+    b <= nb -> n >= a + nb -> a + b <= n.
+  Proof.
+    intros; omega.
+  Qed.
+
+  Local Hint Resolve items_per_val_not_0 items_per_val_gt_0 items_per_val_gt_0'.
+
+  (*
+  Lemma array_rep_synced_app : forall xp start na ta tb a b,
+    length a = na * items_per_val ->
+    array_rep xp start (Synced ta a) *
+    array_rep xp (start + (divup (length a) items_per_val)) (Synced tb b) =p=>
+    array_rep xp start (Synced (ta ++ tb) (a ++ b)).
+  Proof.
+    simpl; intros;
+    unfold synced_array, rep_common, nils; norm; subst; intuition.
+    cancel.
+    erewrite ipack_app by eauto.
+    setoid_rewrite combine_length.
+    repeat rewrite min_r.
+    rewrite app_length, Nat.add_assoc.
+    rewrite <- repeat_app.
+    rewrite combine_app.
+    rewrite arrayN_app. combine_length_eq by auto.
+    repeat rewrite ipack_length.
+    cancel.
+
+    unfold items_valid, roundup in *; intuition.
+    apply well_formed_app_iff; auto.
+    rewrite app_length.
+    eapply helper_add_le; eauto.
+    rewrite Nat.sub_add_distr.
+    setoid_rewrite Nat.mul_sub_distr_r at 2.
+    apply helper_add_sub.
+    apply roundup_ge; auto.
+    apply Nat.mul_le_mono_r; omega.
+
+    erewrite ipack_app; eauto.
+    simplen.
+  Qed.
+
+  Lemma array_rep_synced_app_rev : forall xp start na a b,
+    length a = na * items_per_val ->
+    array_rep xp start (Synced (a ++ b)) =p=>
+    array_rep xp start (Synced a) *
+    array_rep xp (start + (divup (length a) items_per_val)) (Synced b).
+  Proof.
+    simpl; intros;
+    unfold synced_array, rep_common, nils, eqlen; norm; subst; intuition;
+    try rewrite repeat_length; auto.
+    cancel.
+    erewrite ipack_app by eauto.
+    rewrite app_length, Nat.add_assoc.
+    rewrite <- repeat_app.
+    rewrite combine_app, arrayN_app, combine_length_eq by (rewrite repeat_length; auto).
+    repeat rewrite ipack_length.
+    cancel.
+    apply (@items_valid_app xp start a b H1).
+    rewrite H, divup_mul by auto.
+    eapply items_valid_app3; eauto.
+  Qed.
+
+  (** read count blocks starting from the beginning *)
+  Definition read_all xp count cs :=
+    let^ (cs, r) <- read_range (RAStart xp) count iunpack nil cs;;
+    Ret ^(cs, r).
+
+  Theorem read_all_ok : forall xp count cs,
+    {< F d items,
+    PRE:hm         BUFCACHE.rep cs d *
+                   [[ length items = (count * items_per_val)%nat /\
+                      Forall Rec.well_formed items /\ xparams_ok xp ]] *
+                   [[ (F * array_rep xp 0 (Synced items))%pred d ]]
+    POST:hm' RET:^(cs, r)
+                   BUFCACHE.rep cs d *
+                   [[ (F * array_rep xp 0 (Synced items))%pred d ]] *
+                   [[ r = items ]]
+    CRASH:hm'  exists cs', BUFCACHE.rep cs' d
+    >} read_all xp count cs.
+  Proof.
+    unfold read_all.
+    step.
+    rewrite synced_array_is, Nat.add_0_r; cancel.
+    simplen.
+
+    step; subst.
+    rewrite map_fst_combine by simplen.
+    rewrite firstn_oob by simplen.
+    eapply iunpack_ipack; eauto.
+  Qed.
+
+  Lemma vsupd_range_unsync_array : forall xp start items old_vs,
+    items_valid xp start items ->
+    eqlen old_vs (ipack items) ->
+    arrayS (RAStart xp + start) (vsupd_range old_vs (ipack items))
+      =p=> unsync_array xp start items.
+  Proof.
+    intros.
+    unfold vsupd_range, unsync_array, rep_common, ipack.
+    cancel.
+    apply arrayN_unify.
+    rewrite skipn_oob.
+    rewrite app_nil_r.
+    f_equal.
+    simplen.
+    simplen.
+  Qed.
+
+  Lemma vsupd_range_nopad_unsync_array : forall xp start (items : itemlist) old_vs,
+    items_valid xp start items ->
+    length old_vs = divup (length items) items_per_val ->
+    arrayS (RAStart xp + start) (vsupd_range old_vs (nopad_ipack items))
+      =p=> unsync_array xp start items.
+  Proof.
+    unfold vsupd_range, unsync_array, rep_common, eqlen.
+    intros.
+    rewrite nopad_ipack_length in *.
+    rewrite firstn_oob by omega.
+    rewrite skipn_oob by omega.
+    cancel.
+    apply arrayN_unify.
+    rewrite app_nil_r.
+    f_equal.
+    auto using ipack_nopad_ipack_eq.
+    autorewrite with core list. auto.
+  Qed.
+
+  Lemma write_aligned_length_helper : forall n l,
+    n <= length (map block2val (list_chunk l items_per_val item0)) ->
+    n <= divup (length l) items_per_val.
+  Proof.
+    intros; autorewrite with lists in *.
+    erewrite <- list_chunk_length; eauto.
+  Qed.
+  Local Hint Resolve write_aligned_length_helper.
+
+  (** write items from a given block index, 
+      slots following the items will be cleared *)
+  Definition write_aligned xp start (items: itemlist) cs :=
+    let chunks := nopad_list_chunk items items_per_val in
+    cs <- BUFCACHE.write_range ((RAStart xp) + start) (map block2val chunks) cs;
+    Ret cs.
+
+  Theorem write_aligned_ok : forall xp start new cs,
+    {< F d,
+    PRE:hm         BUFCACHE.rep cs d *
+                   [[ items_valid xp start new ]] *
+                   [[ (F * avail_rep xp start (divup (length new) items_per_val))%pred d ]]
+    POST:hm' RET: cs
+                   exists d', BUFCACHE.rep cs d' *
+                   [[ (F * array_rep xp start (Unsync new))%pred d' ]]
+    XCRASH:hm'  exists cs' d',
+                   BUFCACHE.rep cs' d' *
+                   [[ (F * avail_rep xp start (divup (length new) items_per_val)) % pred d' ]]
+    >} write_aligned xp start new cs.
+  Proof.
+    unfold write_aligned, avail_rep.
+    step.
+    cbn. simplen.
+    step.
+    apply vsupd_range_nopad_unsync_array; auto.
+    xcrash.
+    rewrite vsupd_range_length; auto.
+    simplen.
+    setoid_rewrite nopad_list_chunk_length; auto.
+  Qed.
+
+
+  Lemma vssync_range_sync_array : forall xp start items count vsl,
+    items_valid xp start items ->
+    length items = (count * items_per_val)%nat ->
+    length vsl = count ->
+    arrayS (RAStart xp + start) (vssync_range (combine (ipack items) vsl) count)
+      =p=> synced_array xp start items.
+  Proof.
+    unfold synced_array, rep_common; cancel; simplen.
+    unfold vssync_range.
+    rewrite skipn_oob by simplen.
+    rewrite app_nil_r.
+    apply arrayN_unify.
+    rewrite firstn_oob by simplen.
+    rewrite map_fst_combine by simplen.
+    auto.
+  Qed.
+
+  Lemma helper_ipack_length_eq: forall (vsl : list (list valu)) count items,
+    eqlen (ipack items) vsl ->
+    length items = count * items_per_val ->
+    count = length vsl.
+  Proof.
+    intros.
+    replace (length vsl) with (length (ipack items)) by simplen.
+    rewrite ipack_length; simplen.
+  Qed.
+
+  Lemma helper_ipack_length_eq': forall (vsl : list (list valu)) count items,
+    eqlen (ipack items) vsl ->
+    length items = count * items_per_val ->
+    length vsl = count.
+  Proof.
+    intros; apply eq_sym; eapply helper_ipack_length_eq; eauto.
+  Qed.
+
+  Local Hint Resolve helper_ipack_length_eq helper_ipack_length_eq'.
+  Hint Rewrite ipack_length.
+
+  Lemma vssync_range_pimpl : forall xp start items vsl m,
+    length items = (length vsl) * items_per_val ->
+    m <= (length vsl) ->
+    arrayS (RAStart xp + start) (vssync_range (combine (ipack items) vsl) m) =p=>
+    arrayS (RAStart xp + start) (combine (ipack items) (repeat nil m ++ skipn m vsl)).
+  Proof.
+    intros.
+    unfold vssync_range, ipack.
+    apply arrayN_unify.
+    rewrite skipn_combine by simplen.
+    rewrite <- combine_app.
+    f_equal.
+    rewrite <- firstn_map_comm.
+    rewrite map_fst_combine by simplen.
+    rewrite firstn_skipn; auto.
+    simplen.
+    lia.
+  Qed.
+
+
+  (** sync count blocks starting from start *)
+  Definition sync_aligned xp start count cs :=
+    cs <- BUFCACHE.sync_range ((RAStart xp) + start) count cs;
+    Ret cs.
+
+  Theorem sync_aligned_ok : forall xp start count cs,
+    {< F d0 d items,
+    PRE:hm         BUFCACHE.synrep cs d0 d * 
+                   [[ (F * array_rep xp start (Unsync items))%pred d ]] *
+                   [[ length items = (count * items_per_val)%nat ]] *
+                   [[ items_valid xp start items /\ sync_invariant F ]]
+    POST:hm' RET: cs
+                   exists d', BUFCACHE.synrep cs d0 d' *
+                   [[ (F * array_rep xp start (Synced items))%pred d' ]]
+    CRASH:hm'  exists cs', BUFCACHE.rep cs' d0
+    >} sync_aligned xp start count cs.
+  Proof.
+    unfold sync_aligned.
+    prestep. norml.
+    unfold unsync_array, rep_common in *; destruct_lifts.
+
+    cancel.
+    rewrite combine_length_eq by simplen.
+    rewrite ipack_length; simplen.
+
+    step.
+    apply vssync_range_sync_array; eauto.
+  Qed.
+
+  Hint Extern 1 ({{_}} Bind (read_all _ _ _) _) => apply read_all_ok : prog.
+  Hint Extern 1 ({{_}} Bind (write_aligned _ _ _ _) _) => apply write_aligned_ok : prog.
+  Hint Extern 1 ({{_}} Bind (sync_aligned _ _ _ _) _) => apply sync_aligned_ok : prog.
+*)
+End AsyncRecArray.
+
