src/PermDiskLogHdr.v
@@ -1,0 +1,393 @@
+Require Import Arith.
+Require Import Bool.
+Require Import Eqdep_dec.
+Require Import Classes.SetoidTactics.
+Require Import PermHashmap.
+Require Import HashmapProg.
+Require Import Pred PermPredCrash.
+Require Import Omega.
+Require Import Word.
+Require Import Rec.
+Require Import WordAuto.
+Require Import FSLayout.
+Require Import Rounding.
+Require Import List ListUtils.
+Require Import Psatz.
+Require Import PermAsyncRecArray.
+Require Export PermCacheSec.
+
+Import ListNotations.
+
+
+ Module DescSig <: RASig.
+
+    Definition xparams := log_xparams.
+    Definition RAStart := LogDescriptor.
+    Definition RALen := LogDescLen.
+    Definition xparams_ok (xp : xparams) := goodSize addrlen ((RAStart xp) + (RALen xp)).
+
+    Definition itemtype := Rec.WordF addrlen.
+    Definition items_per_val := valulen / addrlen.
+
+    Theorem blocksz_ok : valulen = Rec.len (Rec.ArrayF itemtype items_per_val).
+    Proof.
+      unfold items_per_val; simpl.
+      rewrite valulen_is.
+      cbv; auto.
+    Qed.
+
+  End DescSig.
+
+
+  Module DataSig <: RASig.
+
+    Definition xparams := log_xparams.
+    Definition RAStart := LogData.
+    Definition RALen := LogLen.
+    Definition xparams_ok (xp : xparams) := goodSize addrlen ((RAStart xp) + (RALen xp)).
+
+    Definition itemtype := Rec.WordF valulen.
+    Definition items_per_val := 1.
+
+    Theorem blocksz_ok : valulen = Rec.len (Rec.ArrayF itemtype items_per_val).
+    Proof.
+      unfold items_per_val; simpl.
+      rewrite valulen_is.
+      cbv; auto.
+    Qed.
+
+  End DataSig.
+
+  Module Desc := AsyncRecArray DescSig.
+  Module Data := AsyncRecArray DataSig.
+  Module DescDefs := Desc.Defs.
+  Module DataDefs := Data.Defs.
+
+
+  Definition header_type := Rec.RecF ([("previous_ndesc", Rec.WordF addrlen);
+                                       ("previous_ndata", Rec.WordF addrlen);
+                                       ("ndesc", Rec.WordF addrlen);
+                                       ("ndata", Rec.WordF addrlen);
+                                       ("addr_checksum", Rec.WordF hashlen);
+                                       ("valu_checksum", Rec.WordF hashlen)]).
+  Definition header := Rec.data header_type.
+  Definition hdr := ((nat * nat) * (nat * nat) * (word hashlen * word hashlen))%type.
+  Definition previous_length (header : hdr) := fst (fst header).
+  Definition current_length (header : hdr) := snd (fst header).
+  Definition checksum (header : hdr) := snd header.
+  Definition mk_header (len : hdr) : header :=
+    ($ (fst (previous_length len)),
+     ($ (snd (previous_length len)),
+      ($ (fst (current_length len)),
+       ($ (snd (current_length len)),
+        (fst (checksum len),
+         (snd (checksum len), tt)))))).
+  
+  Theorem hdrsz_ok : Rec.len header_type <= valulen.
+  Proof.
+    rewrite valulen_is. apply leb_complete. compute. trivial.
+  Qed.
+  Local Hint Resolve hdrsz_ok.
+  
+  Lemma plus_minus_header : Rec.len header_type + (valulen - Rec.len header_type) = valulen.
+  Proof.
+    apply le_plus_minus_r; auto.
+  Qed.
+  
+  Definition hdr2val (h : header) : valu.
+    set (zext (Rec.to_word h) (valulen - Rec.len header_type)) as r.
+    rewrite plus_minus_header in r.
+    refine r.
+  Defined.
+  
+  Definition val2hdr (v : valu) : header.
+    apply Rec.of_word.
+    rewrite <- plus_minus_header in v.
+    refine (split1 _ _ v).
+  Defined.
+  
+  Arguments hdr2val: simpl never.
+  
+  Lemma val2hdr2val : forall h,
+                        val2hdr (hdr2val h) = h.
+  Proof.
+    unfold val2hdr, hdr2val.
+    unfold eq_rec_r, eq_rec.
+    intros.
+    rewrite <- plus_minus_header.
+    unfold zext.
+    autorewrite with core; auto.
+    simpl; destruct h; tauto.
+  Qed.
+  
+  Arguments val2hdr: simpl never.
+  Opaque val2hdr.  (* for some reason "simpl never" doesn't work *)
+  
+  
+  Definition xparams := log_xparams.
+  Definition LAHdr := LogHeader.
+  
+  Inductive state : Type :=
+  | Synced : hdr -> state
+  | Unsync : hdr -> hdr -> state
+  .
+  
+  Definition hdr_goodSize header :=
+    goodSize addrlen (fst (previous_length header)) /\
+    goodSize addrlen (snd (previous_length header)) /\
+    goodSize addrlen (fst (current_length header)) /\
+    goodSize addrlen (snd (current_length header)).
+  
+  Definition state_goodSize st :=
+    match st with
+    | Synced n => hdr_goodSize n
+    | Unsync n o => hdr_goodSize n /\ hdr_goodSize o
+    end.
+  
+  Definition rep xp state : @rawpred :=
+    ([[ state_goodSize state ]] *
+     match state with
+     | Synced n =>
+       (LAHdr xp) |+> ((Public, hdr2val (mk_header n)), nil)
+     | Unsync n o =>
+       (LAHdr xp) |+> ((Public, hdr2val (mk_header n)), [(Public, hdr2val (mk_header o))]%list)
+     end)%pred.
+  
+  
+  
+Definition read xp cs := Eval compute_rec in
+      csh <- read (LAHdr xp) cs;;
+      let cs := fst csh in
+      let h := snd csh in    
+      v <- Unseal h;;
+      let header := (val2hdr v) in
+      Ret (cs,
+           ((# (header :-> "previous_ndesc"),
+             # (header :-> "previous_ndata")),
+            (# (header :-> "ndesc"),
+             # (header :-> "ndata")),
+            (header :-> "addr_checksum",
+             header :-> "valu_checksum"))).
+
+Definition write xp n cs :=
+    h <- Seal Public (hdr2val (mk_header n));;
+    cs <- write (LAHdr xp) h cs;;
+    Ret cs.
+
+Definition sync xp cs :=
+  cs <- sync (LAHdr xp) cs;;
+     Ret cs.
+
+Definition sync_now xp cs :=
+  cs <- begin_sync cs;;
+     cs <- PermCacheDef.sync (LAHdr xp) cs;;
+     cs <- end_sync cs;;
+     Ret cs.
+
+Definition init xp cs :=
+  h <- Hash default_valu;;
+    hdr <- Seal Public (hdr2val (mk_header((0, 0), (0, 0), (h, h))));;
+    cs <- PermCacheDef.write (LAHdr xp) hdr cs;;
+    cs <- begin_sync cs;;
+    cs <- PermCacheDef.sync (LAHdr xp) cs;;
+    cs <- end_sync cs;;
+    Ret cs.
+
+Local Hint Unfold rep state_goodSize : hoare_unfold.
+
+Lemma can_access_public_all:
+  forall pr, can_access pr Public.
+Proof.
+  unfold can_access; intros; destruct pr; intuition eauto.
+Qed.
+
+Hint Resolve can_access_public_all.
+
+Theorem write_ok :
+  forall xp n cs pr,
+      {< F d old,
+      PERM:pr   
+      PRE:bm, hm,
+         PermCacheDef.rep cs d bm *
+         [[ hdr_goodSize n ]] *
+         [[ previous_length n = current_length old \/
+         previous_length old = current_length n ]] *
+         [[ (F * rep xp (Synced old))%pred d ]]
+    POST:bm', hm', RET: cs
+         exists d', PermCacheDef.rep cs d' bm' *
+         [[ exists h, bm' = upd bm h (Public, (hdr2val (mk_header n))) ]] *                       
+         [[ (F * rep xp (Unsync n old))%pred d' ]]
+    XCRASH:bm'', hm'',
+         exists cs' d', PermCacheDef.rep cs' d' bm'' * 
+         [[ (F * rep xp (Unsync n old))%pred d' ]]
+    >} write xp n cs.
+Proof.
+  unfold write.
+  step.
+  safestep.
+  rewrite rep_none_upd_pimpl; eauto.
+  apply upd_eq; auto.
+  eauto.
+  eauto.
+  step.
+  step.
+  eexists; repeat (eapply hashmap_subset_trans; eauto).
+  erewrite <- H1; cancel; eauto.
+  eexists; eapply hashmap_subset_trans; eauto.
+  xcrash.
+
+  safestep.
+  rewrite rep_none_upd_pimpl; eauto.
+  apply upd_eq; auto.
+  eauto.
+  eauto.
+  step.
+  step.
+  eexists; repeat (eapply hashmap_subset_trans; eauto).
+  erewrite <- H1; cancel; eauto.
+  eexists; eapply hashmap_subset_trans; eauto.
+  xcrash.
+  Unshelve.
+  all: unfold EqDec; apply handle_eq_dec.
+Qed.
+
+Theorem read_ok :
+ forall xp cs pr,
+ {< F d n,
+ PERM:pr
+ PRE:bm, hm,
+     PermCacheDef.rep cs d bm *
+     [[ (F * rep xp (Synced n))%pred d ]]
+ POST:bm', hm', RET: ^(cs, r)
+     PermCacheDef.rep cs d bm' *
+     [[ (F * rep xp (Synced n))%pred d ]] *
+     [[ r = n ]]
+ CRASH:bm'', hm'',
+     exists cs', PermCacheDef.rep cs' d bm''
+ >} read xp cs.
+Proof.
+  unfold read.
+  hoare.
+  apply upd_eq; auto.
+  subst; rewrite val2hdr2val; simpl.
+  unfold hdr_goodSize in *; intuition.
+  repeat rewrite wordToNat_natToWord_idempotent'; auto.
+  destruct n; auto.
+  destruct p as (p1 , p2); destruct p1, p2, p0; auto.
+  eexists; repeat(eapply hashmap_subset_trans; eauto).
+Qed.
+
+Theorem sync_ok :
+  forall xp cs pr,
+    {< F d0 d n old,
+     PERM:pr
+     PRE:bm, hm,
+       PermCacheDef.synrep cs d0 d bm *
+       [[ (F * rep xp (Unsync n old))%pred d ]] *
+       [[ sync_invariant F ]]
+     POST:bm', hm', RET: cs
+       exists d', PermCacheDef.synrep cs d0 d' bm' *
+       [[ (F * rep xp (Synced n))%pred d' ]]
+    CRASH:bm'', hm'',  exists cs', PermCacheDef.rep cs' d0 bm''
+    >} sync xp cs.
+Proof.
+  unfold sync.
+  safestep.
+  eassign F_; cancel.
+  all: eauto.
+  step.
+  step.
+  eexists; eapply hashmap_subset_trans; eauto.
+Qed.
+
+Theorem sync_now_ok :
+  forall xp cs pr,
+        {< F d n old,
+         PERM:pr
+         PRE:bm, hm,
+                   PermCacheDef.rep cs d bm *
+                   [[ (F * rep xp (Unsync n old))%pred d ]] *
+                   [[ sync_invariant F ]]
+    POST:bm', hm', RET: cs
+                   exists d', PermCacheDef.rep cs d' bm' *
+                   [[ (F * rep xp (Synced n))%pred d' ]]
+    CRASH:bm'', hm'',  exists cs', PermCacheDef.rep cs' d bm''
+    >} sync_now xp cs.
+Proof.
+  unfold sync_now; intros.
+  step.
+  safestep.
+  eassign F_; cancel.
+  all: eauto.
+  safestep.
+  eassign F_; cancel.
+  all: eauto.
+  step.
+  step.
+  eexists; repeat(eapply hashmap_subset_trans; eauto).
+  rewrite <- H1; cancel; eauto.
+  eexists; repeat(eapply hashmap_subset_trans; eauto).
+  rewrite <- H1; cancel; eauto.
+  eexists; repeat(eapply hashmap_subset_trans; eauto).
+Qed.
+
+
+Theorem init_ok :
+  forall xp cs pr,
+    {< F d v0,
+     PERM:pr
+     PRE:bm, hm,
+        PermCacheDef.rep cs d bm*
+        [[ (F * (LAHdr xp) |+> v0)%pred d ]] *
+        [[ sync_invariant F ]]
+     POST:bm', hm', RET: cs
+        exists d', PermCacheDef.rep cs d' bm'*
+         [[ (F * rep xp (Synced ((0, 0), (0, 0),
+                                 (hash_fwd default_valu,
+                                  hash_fwd default_valu))))%pred d' ]]
+     CRASH:bm'', hm'',
+        any
+    >} init xp cs.
+Proof.
+  unfold init, rep; intros.
+  step.
+  step.
+  safestep.
+  rewrite block_mem_subset_rep; eauto.
+  cancel.
+  apply upd_eq; auto.
+  all: eauto.
+  step.
+  safestep.
+  eassign F_; eassign d'; cancel.
+  all: eauto.
+  safestep.
+  eassign F_; eassign d'; cancel.
+  all: eauto.
+  step.
+  step.
+  unfold hdr_goodSize; cbn.
+  repeat split; apply zero_lt_pow2.
+  eexists; repeat (eapply hashmap_subset_trans; eauto).
+  all: rewrite <- H1; cancel;
+  [ apply pimpl_any |
+    eexists; repeat (eapply hashmap_subset_trans; eauto) |
+    unfold pimpl; intros; eauto ].
+  Unshelve.
+  all: unfold EqDec; apply handle_eq_dec.
+Qed.
+
+
+Theorem sync_invariant_rep :
+  forall xp st,
+    sync_invariant (rep xp st).
+Proof.
+  unfold rep; destruct st; eauto.
+Qed.
+
+Hint Resolve sync_invariant_rep.
+Hint Extern 1 ({{_ | _}} Bind (write _ _ _) _) => apply write_ok : prog.
+Hint Extern 1 ({{_ | _}} Bind (read _ _) _) => apply read_ok : prog.
+Hint Extern 1 ({{_ | _}} Bind (sync _ _) _) => apply sync_ok : prog.
+Hint Extern 1 ({{_ | _}} Bind (sync_now _ _) _) => apply sync_now_ok : prog.
+Hint Extern 1 ({{_ | _}} Bind (init _ _) _) => apply init_ok : prog.
